Rename progress to step and add a deprecation warning

backends/lean/Aeneas/Step/Init.lean
@@ -2,54 +2,54 @@ import Lean
 import AeneasMeta.Utils
 import Aeneas.Std.Primitives
 import AeneasMeta.Extensions
-import Aeneas.Progress.Trace
+import Aeneas.Step.Trace
 import Aeneas.Std.WP
 import AeneasMeta.OptionConfig
 
 namespace Aeneas
 
-namespace Progress
+namespace Step
 
 open Lean Elab Term Meta
 open Utils Extensions
 
 /-!
-# Attribute: `progress_simps`
+# Attribute: `step_simps`
 -/
 
-/-- The `progress_simps` simp attribute. -/
-initialize progressSimpExt : SimpExtension ←
-  registerSimpAttr `progress_simps "\
-    The `progress_simps` attribute registers simp lemmas to be used by `progress`
+/-- The `step_simps` simp attribute. -/
+initialize stepSimpExt : SimpExtension ←
+  registerSimpAttr `step_simps "\
+    The `step_simps` attribute registers simp lemmas to be used by `step`
     to simplify the goal before looking up lemmas. If often happens that some
     monadic function calls, if given some specific parameters (in particuler,
     specific trait instances), can be simplified to far simpler functions: this
     is the main purpose of this attribute."
 
 /-!
-# Attribute: `progress_pre_simps`
+# Attribute: `step_pre_simps`
 -/
 
-/-- The `progress_pre_simps` simp attribute. -/
-initialize progressPreSimpExt : SimpExtension ←
-  registerSimpAttr `progress_pre_simps "\
-    The `progress_pre_simps` attribute registers simp lemmas to be used by `progress`
+/-- The `step_pre_simps` simp attribute. -/
+initialize stepPreSimpExt : SimpExtension ←
+  registerSimpAttr `step_pre_simps "\
+    The `step_pre_simps` attribute registers simp lemmas to be used by `step`
     when solving preconditions by means of the simplifier."
 
 /-!
-# Attribute: `progress_post_simps`
+# Attribute: `step_post_simps`
 -/
 
-/-- The `progress_post_simps` simp attribute. -/
-initialize progressPostSimpExt : SimpExtension ←
-  registerSimpAttr `progress_post_simps "\
-    The `progress_post_simps` attribute registers simp lemmas to be used by `progress`
+/-- The `step_post_simps` simp attribute. -/
+initialize stepPostSimpExt : SimpExtension ←
+  registerSimpAttr `step_post_simps "\
+    The `step_post_simps` attribute registers simp lemmas to be used by `step`
     to post-process post-conditions after introducing them in the context."
 
-/-- The `progress_post_simps_proc` simp attribute for the simp rocs. -/
-initialize progressPostSimprocExt : Simp.SimprocExtension ←
-  Simp.registerSimprocAttr `progress_post_simps_proc "\
-    The `progress_post_simps_proc` attribute registers simp procedures to be used by `progress`
+/-- The `step_post_simps_proc` simp attribute for the simp rocs. -/
+initialize stepPostSimprocExt : Simp.SimprocExtension ←
+  Simp.registerSimprocAttr `step_post_simps_proc "\
+    The `step_post_simps_proc` attribute registers simp procedures to be used by `step`
     during its preprocessing phase." none
 
 /-!
@@ -61,7 +61,7 @@ structure Config where
   async : Bool := false
   /-- Attempt to discharge preconditions by matching them against local assumptions. -/
   assumTac : Bool := true
-  /-- Attempt to infer the ghost variables (variables of progress theorems
+  /-- Attempt to infer the ghost variables (variables of step theorems
       that are not bound in the function call). This requires `assumTac` to
       be `true`. -/
   inferGhostVars : Bool := true
@@ -99,11 +99,11 @@ def Config.toGrindConfig (cfg : Config) : Grind.Config :=
         splits, ematch, splitMatch, splitIte, splitIndPred, funext, gen, instances, canonHeartbeats } := cfg
   { splits, ematch, splitMatch, splitIte, splitIndPred, funext, gen, instances, canonHeartbeats }
 
-declare_option_config_elab Config elabPartialConfig aeneas.progress
+declare_option_config_elab Config elabPartialConfig aeneas.step
 
-/-! # Attribute: `progress` -/
+/-! # Attribute: `step` -/
 
-structure ProgressSpecDesc where
+structure StepSpecDesc where
   -- The universally quantified variables and preconditions, as mvars
   preconds : Array MVarId
   -- The existentially quantified variables
@@ -136,21 +136,21 @@ section Methods
     withLocalDeclsD ⟨ tys ⟩ k
 end Methods
 
-/- Analyze a goal or a progress theorem to decompose its arguments.
+/- Analyze a goal or a step theorem to decompose its arguments.
 
-  ProgressSpec theorems should be of the following shape:
+  StepSpec theorems should be of the following shape:
   ```
   ∀ x1 ... xn, H1 → ... Hn → spec (f x1 ... xn) P
   ```
 -/
-def getProgressSpecFunArgsExpr (ty : Expr) :
+def getStepSpecFunArgsExpr (ty : Expr) :
   MetaM Expr := do
   let ty := ty.consumeMData
   unless ← isProp ty do
     throwError "Expected a proposition, got {←inferType ty}"
   -- ty == ∀ xs, spec (f x1 ... xn) P
   let (xs, xs_bi, ty₂) ← forallMetaTelescope ty
-  trace[Progress] "Universally quantified arguments and assumptions: {xs}"
+  trace[Step] "Universally quantified arguments and assumptions: {xs}"
   -- ty₂ == spec (f x1 ... xn) P
   let (spec?, args) := ty₂.consumeMData.withApp (fun f args => (f, args))
   if h: spec?.isConstOf ``Std.WP.spec ∧ args.size = 3
@@ -185,45 +185,45 @@ def mkExtension (name : Name := by exact decl_name%) :
     addEntry    := Rules.insert,
   }
 
-/-- The progress attribute -/
-structure ProgressSpecAttr where
+/-- The step attribute -/
+structure StepSpecAttr where
   attr : AttributeImpl
   ext  : Extension
   deriving Inhabited
 
-private def saveProgressSpecFromThm (ext : Extension) (attrKind : AttributeKind) (thName : Name) :
+private def saveStepSpecFromThm (ext : Extension) (attrKind : AttributeKind) (thName : Name) :
   AttrM Unit := do
   -- Lookup the theorem
   let env ← getEnv
   -- Ignore some auxiliary definitions (see the comments for attrIgnoreMutRec)
   attrIgnoreAuxDef thName (pure ()) do
-    trace[Progress] "Registering `progress` theorem for {thName}"
+    trace[Step] "Registering `step` theorem for {thName}"
     let some thDecl := env.findAsync? thName
       | throwError "Could not find theorem {thName}"
     let type := thDecl.sig.get.type
     let fKey ← MetaM.run' (do
-      trace[Progress] "Theorem: {type}"
+      trace[Step] "Theorem: {type}"
       -- Normalize to eliminate the let-bindings
       let ty ← normalizeLetBindings type
-      trace[Progress] "Theorem after normalization (to eliminate the let bindings): {ty}"
-      let fExpr ← getProgressSpecFunArgsExpr ty
-      trace[Progress] "Registering spec theorem for expr: {fExpr}"
+      trace[Step] "Theorem after normalization (to eliminate the let bindings): {ty}"
+      let fExpr ← getStepSpecFunArgsExpr ty
+      trace[Step] "Registering spec theorem for expr: {fExpr}"
       -- Convert the function expression to a discrimination tree key
       DiscrTree.mkPath fExpr)
     -- Save the entry
     ScopedEnvExtension.add ext (fKey, thName) attrKind
-    trace[Progress] "Saved the entry"
+    trace[Step] "Saved the entry"
     pure ()
 
-/- Initiliaze the `progress` attribute. -/
-initialize progressAttr : ProgressSpecAttr ← do
-  let ext ← mkExtension `progressMap
+/- Initiliaze the `step` attribute. -/
+initialize stepAttr : StepSpecAttr ← do
+  let ext ← mkExtension `stepMap
   let attrImpl : AttributeImpl := {
-    name := `progress
-    descr := "Adds theorems to the `progress` database"
+    name := `step
+    descr := "Adds theorems to the `step` database"
     add := fun thName stx attrKind => do
       Attribute.Builtin.ensureNoArgs stx
-      saveProgressSpecFromThm ext attrKind thName
+      saveStepSpecFromThm ext attrKind thName
     erase := fun thName => do
       let s := ext.getState (← getEnv)
       let s := s.erase thName
@@ -232,26 +232,26 @@ initialize progressAttr : ProgressSpecAttr ← do
   registerBuiltinAttribute attrImpl
   pure { attr := attrImpl, ext := ext }
 
-def ProgressSpecAttr.find? (s : ProgressSpecAttr) (e : Expr) : MetaM (Array Name) := do
+def StepSpecAttr.find? (s : StepSpecAttr) (e : Expr) : MetaM (Array Name) := do
   let state := s.ext.getState (← getEnv)
   let rules ← state.rules.getMatch e
   pure (rules.filter (fun th => th ∉ state.deactivated))
 
-def ProgressSpecAttr.getState (s : ProgressSpecAttr) : MetaM Rules := do
+def StepSpecAttr.getState (s : StepSpecAttr) : MetaM Rules := do
   pure (s.ext.getState (← getEnv))
 
-def showStoredProgressThms : MetaM Unit := do
-  let st ← progressAttr.getState
+def showStoredStepThms : MetaM Unit := do
+  let st ← stepAttr.getState
   -- TODO: how can we iterate over (at least) the values stored in the tree?
   --let s := st.toList.foldl (fun s (f, th) => f!"{s}\n{f} → {th}") f!""
   let s := f!"{st.rules}, {st.deactivated.toArray}"
   IO.println s
 
-/-! # Attribute: `progress_pure` -/
+/-! # Attribute: `step_pure` -/
 
 namespace Test
   /-!
-  Making some tests here as models to guide the automation generation of proof terms when lifting theorems in `progress_pure`
+  Making some tests here as models to guide the automation generation of proof terms when lifting theorems in `step_pure`
   -/
   open Std Result
   def pos_pair : Int × Int := (0, 1)
@@ -393,7 +393,7 @@ def liftThmType (thmTy : Expr) (pat : Option Syntax)
    -/
   (mkPred : Expr → Expr → Expr → Array Expr → MetaM Expr) :
   MetaM Expr := do
-  withTraceNode `Progress (fun _ => pure m!"liftThmType") do
+  withTraceNode `Step (fun _ => pure m!"liftThmType") do
   /- Strip the quantifiers *before* elaborating the pattern -/
   forallTelescope thmTy.consumeMData fun fvars thmTy => do
   let pat ← do
@@ -401,9 +401,9 @@ def liftThmType (thmTy : Expr) (pat : Option Syntax)
     | none => mkPat fvars thmTy
     | some pat => do
       pure ((← Elab.Term.elabTerm pat none |>.run).fst)
-  trace[Progress] "Elaborated pattern: {pat}"
+  trace[Step] "Elaborated pattern: {pat}"
   existsTelescope pat.consumeMData fun _ patEq => do
-  trace[Progress] "patEq: {patEq}"
+  trace[Step] "patEq: {patEq}"
   /- Destruct the equality. Note that there may not be an equality, in which case
      we see the type as a tuple and introduce one variable per field of the tuple
      (and a single variable if it is actually not a tuple). -/
@@ -414,15 +414,15 @@ def liftThmType (thmTy : Expr) (pat : Option Syntax)
       withFreshTupleFieldFVars (.str .anonymous basename) (← inferType pat) fun fvars => do
       k pat (← mkProdsVal fvars.toList)
   tryDestEq "x" patEq fun pat fvarsPat => do
-  trace[Progress] "Decomposed patterns: pat: {pat}, fvarsPat: {fvarsPat}"
+  trace[Step] "Decomposed patterns: pat: {pat}, fvarsPat: {fvarsPat}"
   /- The decomposed pattern should be tuple a expression: decompose it further into a list of variables -/
   let patFVars : Array Expr := ⟨ destProdsVal fvarsPat ⟩
   /- Substitute the pattern -/
   let thmTy ← mkPred thmTy pat fvarsPat fvars
-  trace[Progress] "Theorem after substituting the pattern: {thmTy}"
+  trace[Step] "Theorem after substituting the pattern: {thmTy}"
   /- Create the nested `predn` -/
   let rec mkPredn (fvars : List Expr) : MetaM Expr := do
-    withTraceNode `Progress (fun _ => pure m!"mkPredn: fvars: {fvars}") do
+    withTraceNode `Step (fun _ => pure m!"mkPredn: fvars: {fvars}") do
     match fvars with
     | [] => throwError "Unexpected"
     | [x] =>
@@ -434,15 +434,15 @@ def liftThmType (thmTy : Expr) (pat : Option Syntax)
       trace[Progres] "thm: {thm}"
       mkAppM ``predn #[← mkLambdaFVars #[x] thm]
   let thmTy ← mkPredn patFVars.toList
-  trace[Progress] "result of mkPredn: {thmTy}"
+  trace[Step] "result of mkPredn: {thmTy}"
   /- Add the `spec` -/
   let liftExpr ← mkAppM ``Std.lift #[pat]
-  trace[Progress] "liftExpr: {liftExpr}"
+  trace[Step] "liftExpr: {liftExpr}"
   let thmTy ← mkAppM ``spec #[liftExpr, thmTy]
-  trace[Progress] "thmTy after introducing `spec`: {thmTy}"
+  trace[Step] "thmTy after introducing `spec`: {thmTy}"
   /- Reintroduce the universal quantifiers -/
   let thmTy ← mkForallFVars fvars thmTy
-  trace[Progress] "thmTy after introducing the quantifiers: {thmTy}"
+  trace[Step] "thmTy after introducing the quantifiers: {thmTy}"
   pure thmTy
 
 
@@ -455,17 +455,17 @@ def liftThmReplaceInTy (thm0 pat npat : Expr) (_ : Array Expr) : MetaM Expr := d
 def liftThm (stx : Syntax) (name : Name) (pat : Option (TSyntax `term))
   (mkPat : Array Expr → Expr → MetaM Expr := fun _ _ => failure)
   (mkPred := liftThmReplaceInTy)
-  (suffix : String := "progress_spec")
+  (suffix : String := "step_spec")
   (tacticStx : Option (TSyntax `tactic) := none)
   : MetaM Name := do
-  trace[Progress] "Name: {name}"
+  trace[Step] "Name: {name}"
   let env ← getEnv
   let some decl := env.findAsync? name
     | throwError "Could not find declaration {name}"
   let sig := decl.sig.get
   -- Generate the type of the theorem
   let thmTy ← liftThmType sig.type pat mkPat mkPred
-  trace[Progress] "thmTy: {thmTy}"
+  trace[Step] "thmTy: {thmTy}"
   -- Prove the theorem - we keep things simple by calling a tactic
   let mvar ← mkFreshExprSyntheticOpaqueMVar thmTy
   let tacticStx ← do
@@ -493,83 +493,83 @@ def liftThm (stx : Syntax) (name : Name) (pat : Option (TSyntax `term))
   pure name
 
 /-!
-# Command: `#progress_pure_lift_thm`
+# Command: `#step_pure_lift_thm`
 
 We do not really use it - it is mostly for testing purposes.
 -/
 
-elab stx:"#progress_pure_lift_thm" id:ident pat:term : command => do
+elab stx:"#step_pure_lift_thm" id:ident pat:term : command => do
   Lean.Elab.Command.runTermElabM fun _ => do
   let some cs ← Term.resolveId? id | throwError m!"Unknown id: {id}"
   let name := cs.constName!
   let _ ← liftThm stx name pat
 
 namespace Test
-  #progress_pure_lift_thm pos_pair_is_pos (∃ x y, pos_pair = (x, y))
+  #step_pure_lift_thm pos_pair_is_pos (∃ x y, pos_pair = (x, y))
 
   /--
-info: Aeneas.Progress.Test.pos_pair_is_pos.progress_spec :
+info: Aeneas.Step.Test.pos_pair_is_pos.step_spec :
   Std.lift pos_pair ⦃ x y =>
     match (x, y) with
     | (x, y) => x ≥ 0 ∧ y ≥ 0 ⦄
   -/
   #guard_msgs in
-  #check pos_pair_is_pos.progress_spec
+  #check pos_pair_is_pos.step_spec
 
-  #progress_pure_lift_thm pos_triple_is_pos pos_triple
+  #step_pure_lift_thm pos_triple_is_pos pos_triple
 
   /--
-info: Aeneas.Progress.Test.pos_triple_is_pos.progress_spec :
+info: Aeneas.Step.Test.pos_triple_is_pos.step_spec :
   Std.lift pos_triple ⦃ x.0 x.1 x.2 =>
     match (x.0, x.1, x.2) with
     | (x, y, z) => x ≥ 0 ∧ y ≥ 0 ∧ z ≥ 0 ⦄
   -/
   #guard_msgs in
-  #check pos_triple_is_pos.progress_spec
+  #check pos_triple_is_pos.step_spec
 
   def pos_triple_is_pos' := pos_triple_is_pos
-  #progress_pure_lift_thm pos_triple_is_pos' (∃ z, pos_triple = z)
+  #step_pure_lift_thm pos_triple_is_pos' (∃ z, pos_triple = z)
 
   /--
-info: Aeneas.Progress.Test.pos_triple_is_pos'.progress_spec :
+info: Aeneas.Step.Test.pos_triple_is_pos'.step_spec :
   Std.lift pos_triple ⦃ z =>
     match z with
     | (x, y, z) => x ≥ 0 ∧ y ≥ 0 ∧ z ≥ 0 ⦄
   -/
   #guard_msgs in
-  #check pos_triple_is_pos'.progress_spec
+  #check pos_triple_is_pos'.step_spec
 
-  #progress_pure_lift_thm overflowing_add_eq (overflowing_add x y)
+  #step_pure_lift_thm overflowing_add_eq (overflowing_add x y)
 
   /--
-info: Aeneas.Progress.Test.overflowing_add_eq.progress_spec (x y : U8) :
+info: Aeneas.Step.Test.overflowing_add_eq.step_spec (x y : U8) :
   Std.lift (overflowing_add x y) ⦃ x.0 x.1 => if x.val + y.val > 255 then x.1 = true else x.1 = false ⦄
   -/
   #guard_msgs in
-  #check overflowing_add_eq.progress_spec
+  #check overflowing_add_eq.step_spec
 end Test
 
 /-!
-# Attribute: `#progress_pure`
+# Attribute: `#step_pure`
 -/
 
-syntax (name := progress_pure) "progress_pure" term : attr
+syntax (name := step_pure) "step_pure" term : attr
 
 section
   variable {m : Type → Type} [Monad m] [MonadOptions m] [MonadTrace m] [AddMessageContext m] [MonadError m]
 
   partial def parseCommaSeparated (isTuple : Bool) (stx : Syntax) (acc : Array Syntax := #[]) :
     m (Array Syntax) := do
-    trace[ProgressElab] "parsing comma separated: {stx} with acc: {acc}"
+    trace[StepElab] "parsing comma separated: {stx} with acc: {acc}"
     -- TODO: check if ident
     match stx with
     | `(ident| $name:ident) =>
-      trace[ProgressElab] "is an ident"
+      trace[StepElab] "is an ident"
       pure (acc.push stx)
     | _ =>
-      trace[ProgressElab] "not an ident"
+      trace[StepElab] "not an ident"
       let args := stx.getArgs
-      trace[ProgressElab] "args.size: {args.size}"
+      trace[StepElab] "args.size: {args.size}"
       /- Parsing is not the same if we have `(...)` or `⟨ ... ⟩`:
         - in the first case, the syntax looks like this (we have nested lists): `["x", "," ["y", ...]]`
         - in the second case, the syntax looks like this (the list is flattened): `["x", ",", "y", ...]`
@@ -580,17 +580,17 @@ section
         let arg0 := args[0]
         let arg1 := args[1]
         let arg2 := args[2]
-        trace[ProgressElab] "parsing comma separated:\n- arg0: {arg0}\n- arg1: {arg1}\n- arg2: {arg2}"
+        trace[StepElab] "parsing comma separated:\n- arg0: {arg0}\n- arg1: {arg1}\n- arg2: {arg2}"
         let isComma ← do
           match arg1 with
           | .atom _ "," => pure true
           | _ => pure false
         if isComma then
-          trace[ProgressElab] "arg1 is a comma"
+          trace[StepElab] "arg1 is a comma"
           parseCommaSeparated isTuple arg2 (acc.push arg0)
         else
           -- Maybe we have a tuple: we simply return the current syntax
-          trace[ProgressElab] "arg1 is not a comma"
+          trace[StepElab] "arg1 is not a comma"
           pure (acc.push stx)
       else if not isTuple then
         -- There should be an odd number of elements: element, comma, element, ...
@@ -614,14 +614,14 @@ section
     return the list of identifiers appearing inside the pattern.
 
   Remark: I tried implementing something simpler based on pattern matching but couldn't get it to work. -/
-  partial def getProgressPurePatternIdents (stx : Syntax) : m (Array Ident) := do
-    trace[ProgressElab] "syntax: {stx}"
+  partial def getStepPurePatternIdents (stx : Syntax) : m (Array Ident) := do
+    trace[StepElab] "syntax: {stx}"
     -- Check if this is an identifier
     match stx with
     | `(term| $name:ident) => pure #[name]
     |_ =>
     let args := stx.getArgs
-    trace[ProgressElab] "args.size: {args.size}"
+    trace[StepElab] "args.size: {args.size}"
 
     -- Check if the syntax is `⟨ ... ⟩` or `( ... )`
     if args.size = 0 then throwError "Unsupported pattern syntax: empty syntax"
@@ -637,9 +637,9 @@ section
         | _, _ => (false, false)
       if not isTupleOrRecord then throwError "Unsupported pattern syntax: {stx}"
       let args ← parseCommaSeparated isTuple arg1
-      trace[ProgressElab] "parsed args: {args}"
+      trace[StepElab] "parsed args: {args}"
       -- Recursively decompose
-      let xs ← args.mapM getProgressPurePatternIdents
+      let xs ← args.mapM getStepPurePatternIdents
       -- Flatten
       pure xs.flatten
     else throwError "Unsupported pattern syntax: {stx}"
@@ -647,14 +647,14 @@ section
   open Lean Elab Command Term in
   /-- Command to check that we correctly parse tuples -/
   local elab "#check_elab_pattern" pat:term " as " ids:ident,* : command => do
-    let ids' ← liftTermElabM (getProgressPurePatternIdents pat)
-    trace[ProgressElab] "Identifiers: {ids'.toList}"
+    let ids' ← liftTermElabM (getStepPurePatternIdents pat)
+    trace[StepElab] "Identifiers: {ids'.toList}"
     let ids ← ids.getElems.mapM fun x => do
       match x with
       | `(ident| $name:ident) => pure name
       | _ => throwError "not an identifier: {x}"
     if ids == ids' then
-      trace[ProgressElab] "Success!"
+      trace[StepElab] "Success!"
     else
       throwError "Mismatch! Expected: {ids}, got: {ids'}"
 
@@ -671,35 +671,35 @@ end
 open Elab Term Attribute in
 /-- We desugar patterns of the shape `foo = (x, y, z)` to `∃ x y z, foo = (x, y, z)` in order to bind
     the variables introduced in the right-hand side, allowing us to elaborate the patterns. -/
-def elabProgressPureAttribute (stx : Syntax) : AttrM (TSyntax `term) :=
+def elabStepPureAttribute (stx : Syntax) : AttrM (TSyntax `term) :=
   withRef stx do
     match stx with
-    | `(attr| progress_pure $x = $pat) => do
-      let ids ← getProgressPurePatternIdents pat
+    | `(attr| step_pure $x = $pat) => do
+      let ids ← getStepPurePatternIdents pat
       let term ← ids.foldrM (fun id term => do
         `(term| ∃ $id:ident, $term)
         ) (← `(term| $x = $pat))
       pure term
-    | `(attr| progress_pure $pat) => do pure pat
+    | `(attr| step_pure $pat) => do pure pat
     | _ => throwUnsupportedSyntax
 
-/-- The progress pure attribute -/
-structure ProgressPureSpecAttr where
+/-- The step pure attribute -/
+structure StepPureSpecAttr where
   attr : AttributeImpl
   deriving Inhabited
 
-/-- The `progress_pure` attribute lifts lemmas about pure functions to `progress` lemmas.
+/-- The `step_pure` attribute lifts lemmas about pure functions to `step` lemmas.
 
-   For instance, if we annotate the following theorem with `progress_pure`:
+   For instance, if we annotate the following theorem with `step_pure`:
    ```lean
-   @[progress_pure wrapping x y]
+   @[step_pure wrapping x y]
    theorem U32.wrapping_add_eq (x y : U32) :
     (wrapping_add x y).bv = x.bv + y.bv
    ```
-   `progress_pure` performs operations which are equivalent to introducing the following lemma:
+   `step_pure` performs operations which are equivalent to introducing the following lemma:
    ```lean
-   @[progress]
-   theorem U32.wrapping_add_eq.progress_spec (x y : U32) :
+   @[step]
+   theorem U32.wrapping_add_eq.step_spec (x y : U32) :
     ↑(wrapping_add x y) ⦃ z => z.bv = x.bv + y.bv ⦄
    ```
 
@@ -707,111 +707,111 @@ structure ProgressPureSpecAttr where
    by writing an equality in the pattern we want to abstract over.
    For instance if we write:
    ```lean
-   @[progress_pure pos_pair = (x, y)]
+   @[step_pure pos_pair = (x, y)]
    theorem pos_pair_is_pos : pos_pair.fst ≥ 0 ∧ pos_pair.snd ≥ 0
    ```
    we get:
    ```lean
-   @[progress]
-   theorem pos_pair_is_pos.progress_spec :
+   @[step]
+   theorem pos_pair_is_pos.step_spec :
     ↑pos_pair ⦃ x y => x ≥ 0 ∧ y ≥ 0 ⦄
    ```
 
    Similarly if we write:
    ```lean
-   @[progress_pure pos_pair = z]
+   @[step_pure pos_pair = z]
    theorem pos_pair_is_pos : pos_pair.fst ≥ 0 ∧ pos_pair.snd ≥ 0
    ```
    we get:
    ```lean
-   @[progress]
-   theorem pos_pair_is_pos.progress_spec :
+   @[step]
+   theorem pos_pair_is_pos.step_spec :
     ↑pos_pair ⦃ z => z.fst ≥ 0 ∧ z.fst ≥ 0 ⦄
    ```
 
-   If we don't put an equality in the pattern, `progress_pure` will introduce one variable
+   If we don't put an equality in the pattern, `step_pure` will introduce one variable
    per field in the type of the pattern, if it is a tuple.
  -/
-initialize progressPureAttribute : ProgressPureSpecAttr ← do
+initialize stepPureAttribute : StepPureSpecAttr ← do
   let attrImpl : AttributeImpl := {
-    name := `progress_pure
-    descr := "Adds lifted version of pure theorems to the `progress_pure` database"
+    name := `step_pure
+    descr := "Adds lifted version of pure theorems to the `step_pure` database"
     add := fun thName stx attrKind => do
       -- Lookup the theorem
       let env ← getEnv
       -- Ignore some auxiliary definitions (see the comments for attrIgnoreMutRec)
       attrIgnoreAuxDef thName (pure ()) do
         -- Elaborate the pattern
-        let pat ← elabProgressPureAttribute stx
+        let pat ← elabStepPureAttribute stx
         -- Introduce the lifted theorem
         let liftedThmName ← MetaM.run' (liftThm stx thName pat)
-        -- Save the lifted theorem to the `progress` database
-        saveProgressSpecFromThm progressAttr.ext attrKind liftedThmName
+        -- Save the lifted theorem to the `step` database
+        saveStepSpecFromThm stepAttr.ext attrKind liftedThmName
   }
   registerBuiltinAttribute attrImpl
   pure { attr := attrImpl }
 
-/-! # Attribute: `progress_pure_def` -/
+/-! # Attribute: `step_pure_def` -/
 
-/-- Automatically generate a `progress` theorem from a pure definition.
+/-- Automatically generate a `step` theorem from a pure definition.
 
 Example:
 ```lean
-@[progress_pure_def wrapping_add = (b, x)]
+@[step_pure_def wrapping_add = (b, x)]
 def wrapping_add (x y : U32) : Bool × U32 := ...
 ```
 generates the theorem:
 ```lean
-@[progress]
-theorem wrapping_add.progress_spec (x y : U32) :
+@[step]
+theorem wrapping_add.step_spec (x y : U32) :
   (lift (wrapping_add x y)) ⦃ b x => (b, x) = wrapping_add x y ⦄
 ```
-(note that the `z` appearing in the post-condition is eliminated when calling `progress`,
+(note that the `z` appearing in the post-condition is eliminated when calling `step`,
 leaving only `b` and `x` in the environment).
  -/
-syntax (name := progress_pure_def) "progress_pure_def" (term)? : attr
+syntax (name := step_pure_def) "step_pure_def" (term)? : attr
 
 /-- We desugar patterns of the shape `foo = (x, y, z)` to `∃ x y z, foo = (x, y, z)` in order to bind
     the variables introduced in the right-hand side, allowing us to elaborate the patterns. -/
-def elabProgressPureDefPattern (stx : Syntax) : AttrM (TSyntax `term) :=
+def elabStepPureDefPattern (stx : Syntax) : AttrM (TSyntax `term) :=
   withRef stx do
     match stx with
     | `(term| $x = $pat)
     | `(term| ($x = $pat)) => do
-      trace[ProgressElab] "elabProgressPureDefPattern: equality pattern"
-      let ids ← getProgressPurePatternIdents pat
+      trace[StepElab] "elabStepPureDefPattern: equality pattern"
+      let ids ← getStepPurePatternIdents pat
       let term ← ids.foldrM (fun id term => do
         `(term| ∃ $id:ident, $term)
         ) (← `(term| $x = $pat))
       pure term
     | `(term| $pat) => do
-      trace[ProgressElab] "elabProgressPureDefPattern: not an equality"
+      trace[StepElab] "elabStepPureDefPattern: not an equality"
       pure pat
 
-/-- The progress pure def attribute -/
-structure ProgressPureDefSpecAttr where
+/-- The step pure def attribute -/
+structure StepPureDefSpecAttr where
   attr : AttributeImpl
   deriving Inhabited
 
 theorem specLiftDef {α} (x : α) : Std.WP.spec (Std.lift x) (fun y => y = x) := by
   simp only [Std.lift, Std.WP.spec_ok]
 
-def mkProgressPureDefThm (stx : Syntax) (pat : Option (TSyntax `term)) (n : Name)
-  (suffix : String := "progress_spec") : MetaM Name := do
+def mkStepPureDefThm (stx : Syntax) (pat : Option (TSyntax `term)) (n : Name)
+  (suffix : String := "step_spec") : MetaM Name := do
   -- Regular case
   let mkPat (fvars : Array Expr) (ty : Expr) : MetaM Expr := do
-    withTraceNode `Progress (fun _ => pure m!"mkPat") do
+    withTraceNode `Step (fun _ => pure m!"mkPat") do
     withLocalDeclD (← mkFreshUserName `x) ty fun v => do
     let x ← mkAppOptM n (fvars.map some)
-    trace[Progress] "x: {x}"
+    trace[Step] "x: {x}"
     let eq ← mkEq x v
-    trace[Progress] "eq: {eq}"
+    trace[Step] "eq: {eq}"
     let eq ← mkLambdaFVars #[v] eq
     let eq ← mkAppM ``Exists #[eq]
-    trace[Progress] "eq: {eq}"
+    trace[Step] "eq: {eq}"
     pure eq
   let mkPred (_ _ npat : Expr) (fvars : Array Expr) : MetaM Expr := do
-    withTraceNode `Progress (fun _ => pure m!"mkPred") do
+    withTraceNode `Step (fun _ => pure m!"mkPred") do
     mkEq npat (← mkAppOptM n (fvars.map some))
   let tacticStx ←
     `(tactic|
@@ -819,64 +819,63 @@ def mkProgressPureDefThm (stx : Syntax) (pat : Option (TSyntax `term)) (n : Name
           [_root_.Aeneas.Std.lift, _root_.Aeneas.Std.WP.spec_ok, _root_.Aeneas.Std.WP.predn, _root_.implies_true])
   liftThm stx n pat mkPat mkPred suffix (tacticStx := some tacticStx)
 
-local elab "#progress_pure_def" id:ident pat:(term)? : command => do
+local elab "#step_pure_def" id:ident pat:(term)? : command => do
   Lean.Elab.Command.runTermElabM (fun _ => do
     let some cs ← Term.resolveId? id | throwError m!"Unknown id: {id}"
     let name := cs.constName!
-    trace[ProgressElab] "pat: {pat}"
+    trace[StepElab] "pat: {pat}"
     let pat ← match pat with
-      | some p => do pure (some (← elabProgressPureDefPattern p))
+      | some p => do pure (some (← elabStepPureDefPattern p))
       | none => pure none
-    let _ ← mkProgressPureDefThm id pat name
+    let _ ← mkStepPureDefThm id pat name
   )
 
 namespace Test
-  #progress_pure_def overflowing_add
-  #elab overflowing_add.progress_spec
+  #step_pure_def overflowing_add
+  #elab overflowing_add.step_spec
 
   /--
-info: Aeneas.Progress.Test.overflowing_add.progress_spec (x y : U8) :
+info: Aeneas.Step.Test.overflowing_add.step_spec (x y : U8) :
   Std.lift (overflowing_add x y) ⦃ x✝ => x✝ = overflowing_add x y ⦄
   -/
   #guard_msgs in
-  #check overflowing_add.progress_spec
+  #check overflowing_add.step_spec
 
   def wrapping_add (x y : U8) : U8 × Bool := (⟨ x.val + y.val ⟩, x.val + y.val ≥ 256)
-  #progress_pure_def wrapping_add (wrapping_add x y = (b, z))
+  #step_pure_def wrapping_add (wrapping_add x y = (b, z))
 
   /--
-info: Aeneas.Progress.Test.wrapping_add.progress_spec (x y : U8) :
-  Std.lift (wrapping_add x y) ⦃ b z => (b, z) = wrapping_add x y ⦄
+info: Aeneas.Step.Test.wrapping_add.step_spec (x y : U8) : Std.lift (wrapping_add x y) ⦃ b z => (b, z) = wrapping_add x y ⦄
   -/
   #guard_msgs in
-  #check wrapping_add.progress_spec
+  #check wrapping_add.step_spec
 end Test
 
-def elabProgressPureDefAttribute (stx : Syntax) : AttrM (Option (TSyntax `term)) :=
+def elabStepPureDefAttribute (stx : Syntax) : AttrM (Option (TSyntax `term)) :=
   withRef stx do
     match stx with
-    | `(attr| progress_pure_def $x = $pat)
-    | `(attr| progress_pure_def ($x = $pat)) => do
-      trace[ProgressElab] "elabProgressPureDefAttribute: equality pattern"
-      let ids ← getProgressPurePatternIdents pat
+    | `(attr| step_pure_def $x = $pat)
+    | `(attr| step_pure_def ($x = $pat)) => do
+      trace[StepElab] "elabStepPureDefAttribute: equality pattern"
+      let ids ← getStepPurePatternIdents pat
       let term ← ids.foldrM (fun id term => do
         `(term| ∃ $id:ident, $term)
         ) (← `(term| $x = $pat))
       pure (some term)
-    | `(attr| progress_pure_def $pat) => do
-      trace[ProgressElab] "elabProgressPureDefAttribute: not an equality"
+    | `(attr| step_pure_def $pat) => do
+      trace[StepElab] "elabStepPureDefAttribute: not an equality"
       pure (some pat)
-    | `(attr| progress_pure_def) => do
-      trace[ProgressElab] "elabProgressPureDefAttribute: not an equality"
+    | `(attr| step_pure_def) => do
+      trace[StepElab] "elabStepPureDefAttribute: not an equality"
       pure none
     | _ => throwError "Unsupported syntax"
 
-/- The `progress_pure_def` attribute, which automatically generates
-   progress lemmas for pure definitions. -/
-initialize progressPureDefAttribute : ProgressPureDefSpecAttr ← do
+/- The `step_pure_def` attribute, which automatically generates
+   step lemmas for pure definitions. -/
+initialize stepPureDefAttribute : StepPureDefSpecAttr ← do
   let attrImpl : AttributeImpl := {
-    name := `progress_pure_def
-    descr := "Automatically generate `progress` theorems for pure definitions"
+    name := `step_pure_def
+    descr := "Automatically generate `step` theorems for pure definitions"
     add := fun declName stx attrKind => do
       -- Lookup the theorem
       let env ← getEnv
@@ -884,15 +883,15 @@ initialize progressPureDefAttribute : ProgressPureDefSpecAttr ← do
       attrIgnoreAuxDef declName (pure ()) do
       -- Elaborate the pattern
         trace[Saturate.attribute] "Syntax: {stx}"
-        let pat ← elabProgressPureDefAttribute stx
+        let pat ← elabStepPureDefAttribute stx
         -- Introduce the lifted theorem
-        let thmName ← MetaM.run' (mkProgressPureDefThm stx pat declName)
-        -- Save the lifted theorem to the `progress` database
-        saveProgressSpecFromThm progressAttr.ext attrKind thmName
+        let thmName ← MetaM.run' (mkStepPureDefThm stx pat declName)
+        -- Save the lifted theorem to the `step` database
+        saveStepSpecFromThm stepAttr.ext attrKind thmName
   }
   registerBuiltinAttribute attrImpl
   pure { attr := attrImpl }
 
-end Progress
+end Step
 
 end Aeneas
