backends/lean/Aeneas/Step/Step.lean
@@ -1,6 +1,6 @@
 import Lean
 import Aeneas.ScalarTac
-import Aeneas.Progress.Init
+import Aeneas.Step.Init
 import Aeneas.Std
 import Aeneas.FSimp
 import AeneasMeta.Async
@@ -8,15 +8,15 @@ import Aeneas.Grind.Init
 
 namespace Aeneas
 
-namespace Progress
+namespace Step
 
 open Lean Elab Term Meta Tactic
 open Utils
 
 /-- A special definition that we use to introduce pretty-printed terms in the context.
 
-Note that we should have `α = β`, but we allow the types to not be equal in case `progress` has
-a bug and doesn't give the proper arguments: this way we make sure tactics like `progress*?`
+Note that we should have `α = β`, but we allow the types to not be equal in case `step` has
+a bug and doesn't give the proper arguments: this way we make sure tactics like `step*?`
 will not crash if there is a bug in the code which adds the pretty equality (this is only useful
 information for the user).
 -/
@@ -33,9 +33,9 @@ def eq_imp_prettyMonadEq {α : Type u} {β : Type v} (x : Std.Result α) (y : β
   unfold prettyMonadEq
   constructor
 
-def traceGoalWithNode (msg : String) : TacticM Unit := Utils.traceGoalWithNode `Progress msg
+def traceGoalWithNode (msg : String) : TacticM Unit := Utils.traceGoalWithNode `Step msg
 
--- TODO: the scalar types annoyingly often get reduced when we use the progress
+-- TODO: the scalar types annoyingly often get reduced when we use the step
 -- tactic. We should find a way of controling reduction. For now we use rewriting
 -- lemmas to make sure the goal remains clean, but this complexifies proof terms.
 -- It seems there used to be a `fold` tactic. Update: there is a `refold_let` in Mathlib
@@ -61,7 +61,7 @@ def scalar_eqs := #[
 want to introduce in the context -/
 theorem forall_unit {p : Prop} : (Unit → p) ↔ p := by simp
 
-attribute [progress_simps]
+attribute [step_simps]
   bind_assoc Std.bind_tc_ok Std.bind_tc_fail Std.bind_tc_div
   /- Those are quite useful to simplify the goal further by eliminating existential quantifiers for instance. -/
   and_assoc Std.Result.ok.injEq Prod.mk.injEq
@@ -70,7 +70,7 @@ attribute [progress_simps]
   -- This one gets only applied to full applications of `predn`, which are typically revealed after applying `spec_ok`
   Std.WP.predn_eq
 
-attribute [progress_post_simps]
+attribute [step_post_simps]
   -- We often see expressions like `Int.ofNat 3`
   Int.reduceToNat
 
@@ -87,7 +87,7 @@ instance : Coe TheoremOrLocal Name where
 inductive UsedTheorem where
   | givenExpr: Expr → UsedTheorem
   | localHyp: LocalDecl → UsedTheorem
-  | progressThm : Name → UsedTheorem
+  | stepThm : Name → UsedTheorem
 
 namespace UsedTheorem
 
@@ -95,14 +95,14 @@ instance: ToString UsedTheorem where
   toString
   | .givenExpr _e => "given expression"
   | .localHyp decl => s!"local hypothesis {decl.userName.toString}"
-  | .progressThm name => s!"progress theorem {name}"
+  | .stepThm name => s!"step theorem {name}"
 
 def toSyntax: UsedTheorem → MetaM Syntax.Term
 | givenExpr e =>
   -- Remark: exprToSyntax doesn't give the expected result
   Lean.Meta.Tactic.TryThis.delabToRefinableSyntax e
 | localHyp decl    => pure <| mkIdent decl.userName
-| progressThm name => do
+| stepThm name => do
   /- Unresolve the name to make sure that the name is valid, and it is
      as short as possible -/
   let name ← Lean.unresolveNameGlobalAvoidingLocals name
@@ -111,7 +111,7 @@ def toSyntax: UsedTheorem → MetaM Syntax.Term
 def getType: UsedTheorem -> MetaM (Option Expr)
 | givenExpr e => inferType e
 | localHyp decl =>inferType decl.toExpr
-| progressThm name => do
+| stepThm name => do
   if let some cinfo := (←getEnv).find? name then
     let expr := cinfo.value! (allowOpaque := true)
     inferType expr
@@ -120,7 +120,7 @@ def getType: UsedTheorem -> MetaM (Option Expr)
 
 end UsedTheorem
 
-/-- Information about a variable introduced by `progress` (output or post-condition). -/
+/-- Information about a variable introduced by `step` (output or post-condition). -/
 structure Output where
   /-- The variable introduced in the context -/
   fvarId : FVarId
@@ -131,7 +131,7 @@ structure Output where
 
 structure MainGoal where
   goal : MVarId
-  /-- The variables introduced in the context after applying the progress theorem (this includes variables "output"
+  /-- The variables introduced in the context after applying the step theorem (this includes variables "output"
       by the monadic function call as well as post-conditions). -/
   outputs : Array Output
 
@@ -170,7 +170,7 @@ deriving Inhabited
 structure Stats extends Goals where
   usedTheorem : UsedTheorem
 
-attribute [progress_post_simps]
+attribute [step_post_simps]
   Std.IScalar.toNat Std.UScalar.ofNatCore_val_eq Std.IScalar.ofInt_val_eq
 
 structure Args where
@@ -218,10 +218,10 @@ def getFirstBind (goalTy : Expr) : MetaM (Bool × Expr) := do
                then pure (args[1])
                else throwError "Goal is not a `spec m P`"
 
-  trace[Progress] "compTy: {compTy}"
+  trace[Step] "compTy: {compTy}"
 
   let (bind?, args) := compTy.consumeMData.withApp (fun f args => (f, args))
-  trace[Progress] "bind?: {bind?}"
+  trace[Step] "bind?: {bind?}"
   if h: bind?.isConstOf ``bind ∧ args.size = 6
   then pure (true, args[4])
   else pure (false, compTy)
@@ -288,7 +288,7 @@ def getPostNamesFromGoal : TacticM (Array (Option Name)) := do
     else pure #[]
   catch _ => pure #[]
 
-/-- Extract variable names from the current goal for naming `progress` outputs.
+/-- Extract variable names from the current goal for naming `step` outputs.
     If the goal is a bind (`let x ← ...`), extracts the binding name.
     Otherwise, extracts names from the post-condition. -/
 def getVarNamesFromGoal : TacticM (Array (Option Name) × Option Name) := do
@@ -300,31 +300,31 @@ def getVarNamesFromGoal : TacticM (Array (Option Name) × Option Name) := do
 
 /-- Attempt to resolve typeclasses. -/
 def trySolveTypeclasses (mvarsIds : List MVarId) : TacticM (List MVarId) := do
-  withTraceNode `Progress (fun _ => pure m!"trySolveTypeclasses") do
+  withTraceNode `Step (fun _ => pure m!"trySolveTypeclasses") do
   mvarsIds.filterMapM fun (mvar : MVarId) => do
-    trace[Progress] "goal: {mvar}"
+    trace[Step] "goal: {mvar}"
     let ty ← instantiateMVars (← mvar.getType)
     ty.withApp fun app _ => do
     if let some (name, _) := app.const? then
-      trace[Progress] "Checking application: {name}"
+      trace[Step] "Checking application: {name}"
       if not (← isProp (← inferType ty)) then
         /- We eagerly consider the application to be a typeclass
            TODO: this might be dangerous -/
-        trace[Progress] "not a prop"
+        trace[Step] "not a prop"
         try
           mvar.withContext do
           let inst ← synthInstance ty
-          trace[Progress] "Solved the typeclass"
+          trace[Step] "Solved the typeclass"
           let _ ← isDefEq (.mvar mvar) inst
           pure none
         catch _ =>
-          trace[Progress] "Could not solve the typeclass"
+          trace[Step] "Could not solve the typeclass"
           pure mvar
       else
-        trace[Progress] "Ignoring a prop"
+        trace[Step] "Ignoring a prop"
         pure mvar
     else
-      trace[Progress] "Could not decompose application"
+      trace[Step] "Could not decompose application"
       pure mvar
 
 /-- Attempt to match a given theorem with the monadic call in the target.
@@ -333,7 +333,7 @@ The resulting target should be of the shape:
 -/
 def tryMatch (isLet : Bool) (th : Expr) :
   TacticM (Array MVarId) := do
-  withTraceNode `Progress (fun _ => pure m!"tryMatch") do
+  withTraceNode `Step (fun _ => pure m!"tryMatch") do
   /- Apply the theorem
      We try to match the theorem with the goal
      In order to match the theorem with the goal, we introduce meta-variables for all
@@ -342,15 +342,15 @@ def tryMatch (isLet : Bool) (th : Expr) :
   /- There might be meta-variables in the type if the theorem comes from a local declaration,
      especially if this declaration was introduced by a tactic -/
   let thTy ← instantiateMVars (← inferType th)
-  trace[Progress] "Looked up theorem/assumption type: {thTy}"
+  trace[Step] "Looked up theorem/assumption type: {thTy}"
   -- Normalize to inline the let-bindings
   let thTy ← normalizeLetBindings thTy
-  trace[Progress] "After normalizing the let-bindings: {thTy}"
-  trace[Progress] "Theorem: {th}: {← inferType th}"
+  trace[Step] "After normalizing the let-bindings: {thTy}"
+  trace[Step] "Theorem: {th}: {← inferType th}"
   -- Introduce the meta-variables for the quantified parameters
   let (mvars, _, thTy) ← forallMetaTelescope thTy
   let th := mkAppN th mvars
-  trace[Progress] "Uninstantiated theorem: {th}: {← inferType th}"
+  trace[Step] "Uninstantiated theorem: {th}: {← inferType th}"
 
   -- `thTy` should be of the shape `spec program post`: we need to retrieve `program`
   let (thHead, thArgs) := thTy.consumeMData.withApp (fun f args => (f, args))
@@ -367,32 +367,32 @@ def tryMatch (isLet : Bool) (th : Expr) :
     else (``Std.WP.spec_mono', 2)
   let specMonoBind ← Term.mkConst specMonoBindName
   let specMonoBindTy ← inferType specMonoBind
-  trace[Progress] "specMonoBind (isLet:{isLet}): {specMonoBind}: {← inferType specMonoBind}"
+  trace[Step] "specMonoBind (isLet:{isLet}): {specMonoBind}: {← inferType specMonoBind}"
   let (specMonoBindMVars, _, specMonoBindTy) ← forallMetaBoundedTelescope specMonoBindTy varNum
   let specMonoBind ← mkAppOptM' specMonoBind (specMonoBindMVars.map some)
-  trace[Progress] "Uninstantiated specMonoBind: {specMonoBind}: {← inferType specMonoBind}"
+  trace[Step] "Uninstantiated specMonoBind: {specMonoBind}: {← inferType specMonoBind}"
 
   let specMonoBind := mkAppN specMonoBind #[program, P, th]
   let specMonoBindTy ← inferType specMonoBind
-  trace[Progress] "Applied specMonoBind with theorem: {specMonoBind}: {specMonoBindTy}"
+  trace[Step] "Applied specMonoBind with theorem: {specMonoBind}: {specMonoBindTy}"
 
   let (specMonoBindMVars, _, specMonoBindTy) ← forallMetaBoundedTelescope specMonoBindTy 1
   if (specMonoBindMVars.size ≠ 1) then throwError "Unreachable"
   let ngoal := specMonoBindMVars[0]!.mvarId!
   let specMonoBind ← mkAppOptM' specMonoBind (specMonoBindMVars.map some)
-  trace[Progress] "Applied specMonoBind with theorem: {specMonoBind}: {specMonoBindTy}"
+  trace[Step] "Applied specMonoBind with theorem: {specMonoBind}: {specMonoBindTy}"
 
   let mgoal ← Tactic.getMainGoal
   let specMonoBindTy ← inferType specMonoBind
   let goalTy ← mgoal.getType
-  trace[Progress] "About to check defeq:\n- specMonoBindTy: {specMonoBindTy}\n- goalTy: {goalTy}"
+  trace[Step] "About to check defeq:\n- specMonoBindTy: {specMonoBindTy}\n- goalTy: {goalTy}"
   let ok ← isDefEq specMonoBindTy goalTy
   if ¬ ok then
-    trace[Progress] "Could not unify the theorem with the target"
+    trace[Step] "Could not unify the theorem with the target"
     throwError "Could not unify the theorem with the target:\n- theorem: {specMonoBindTy}\n- target: {goalTy}"
 
   mgoal.assign specMonoBind
-  trace[Progress] "New goal: {ngoal}"
+  trace[Step] "New goal: {ngoal}"
 
   let env ← getEnv
   let mvarsIds := mvars.map Expr.mvarId!
@@ -411,22 +411,22 @@ def tryMatch (isLet : Bool) (th : Expr) :
 /-- Small helper: introduce the pretty equality (e.g., `[> let z ← x + y <]`) -/
 def introPrettyEquality (args : Args) (fExpr : Expr) (outputFVars : Array Expr) :
   TacticM Unit := do
-  withTraceNode `Progress (fun _ => pure m!"introPrettyEquality") do
+  withTraceNode `Step (fun _ => pure m!"introPrettyEquality") do
   withMainContext do
-  trace[Progress] "fExpr: {fExpr},\noutputFVars: {outputFVars}"
+  trace[Step] "fExpr: {fExpr},\noutputFVars: {outputFVars}"
   let some name := args.keepPretty
     | return
   -- Construct the tuple of outputs
   let pat ← mkProdsVal outputFVars.toList
-  trace[Progress] "Constructed the pattern: {pat}"
+  trace[Step] "Constructed the pattern: {pat}"
   -- Create the equality
   let e ← mkAppM ``eq_imp_prettyMonadEq #[fExpr, pat]
-  trace[Progress] "Created the equality expression: {e}"
+  trace[Step] "Created the equality expression: {e}"
   -- Introduce it
   Utils.addDeclTac name e (← inferType e) (asLet := false) fun e => do
-    trace[Progress] "Introduced the \"pretty\" let binding: {← inferType e}"
+    trace[Step] "Introduced the \"pretty\" let binding: {← inferType e}"
 
-/-- After application of the progress theorem, the target should be of the shape:
+/-- After application of the step theorem, the target should be of the shape:
   `qimp_spec P k Q` (or `qimp P Q`)
 
   We transform it to a target of the shape:
@@ -440,42 +440,42 @@ def introPrettyEquality (args : Args) (fExpr : Expr) (outputFVars : Array Expr) 
 -/
 def introOutputs (args : Args) (fExpr : Expr) :
   TacticM (Option MainGoal) := do
-  withTraceNode `Progress (fun _ => pure m!"introOutputs") do
+  withTraceNode `Step (fun _ => pure m!"introOutputs") do
   /- Decompose nested uses of `predn` to introduce a sequence of universal quantifiers.
      Note that at the same time we simplify the (monadic) continuation by using
      some monad simp theorems. -/
-  let some _ ← withTraceNode `Progress (fun _ => pure m!"simpAt: decomposing nested uses of `predn`") do
+  let some _ ← withTraceNode `Step (fun _ => pure m!"simpAt: decomposing nested uses of `predn`") do
     Simp.simpAt true { maxDischargeDepth := 1, failIfUnchanged := false, iota := false}
-            { simpThms := #[← progressSimpExt.getTheorems],
+            { simpThms := #[← stepSimpExt.getTheorems],
               addSimpThms :=
                 #[``Std.WP.qimp_spec_predn, ``Std.WP.qimp_spec_unit,
                   ``Std.WP.qimp_predn, ``Std.WP.qimp_unit,
                   ``Std.WP.qimp_spec_exists, ``Std.WP.qimp_exists,
                   ``forall_unit, ``true_imp_iff] }
             (.targets #[] true)
-    | trace[Progress] "The main goal was solved!"; return none
+    | trace[Step] "The main goal was solved!"; return none
   traceGoalWithNode "goal after decomposing the nested `predn`"
 
   /- Eliminate `qimp_spec`/`qimp` to reveal `imp` and decompose the post-condition into a sequence
      of implications -/
-  let some _ ← withTraceNode `Progress (fun _ => pure m!"simpAt: eliminating `qimp_spec` and `qimp`") do
+  let some _ ← withTraceNode `Step (fun _ => pure m!"simpAt: eliminating `qimp_spec` and `qimp`") do
     Simp.simpAt true { maxDischargeDepth := 1, failIfUnchanged := false, iota := false}
             { declsToUnfold := #[``Std.WP.curry, ``Std.WP.predn]
               addSimpThms :=
                 #[``Std.WP.qimp_spec_iff, ``Std.WP.qimp_iff,
                   ``Std.WP.imp_and_iff, ``forall_unit, ``true_imp_iff] }
             (.targets #[] true)
-    | trace[Progress] "The main goal was solved!"; return none
+    | trace[Step] "The main goal was solved!"; return none
   traceGoalWithNode "goal after aliminating `qimp_spec` and `qimp` and decomposing the post-condition"
 
   /- Eliminate `imp`
 
   Some types get unfolded too much (e.g., `U32` sometimes gets unfolded to `U32) so we use this call
   to `dsimp` to also fold them back. -/
-  withTraceNode `Progress (fun _ => pure m!"dsimpAt: eliminating `imp` and folding back scalar types") do
+  withTraceNode `Step (fun _ => pure m!"dsimpAt: eliminating `imp` and folding back scalar types") do
     Simp.dsimpAt true {implicitDefEqProofs := true, failIfUnchanged := false, iota := false}
       { declsToUnfold := #[``Std.WP.imp], addSimpThms := scalar_eqs } (.targets #[] true)
-  if (← getUnsolvedGoals).isEmpty then trace[Progress] "The main goal was solved!"; return none
+  if (← getUnsolvedGoals).isEmpty then trace[Step] "The main goal was solved!"; return none
   traceGoalWithNode "goal after aliminating `imp` and folding back the scalar types"
 
   /- Introduce the outputs.
@@ -503,14 +503,14 @@ def introOutputs (args : Args) (fExpr : Expr) :
     match i? with
     | none => (nFVars, 0)
     | some i => (i, nFVars - i)
-  trace[Progress] "Prefix length: {prefixLength}, post-fix length: {postFixLength}"
+  trace[Step] "Prefix length: {prefixLength}, post-fix length: {postFixLength}"
 
   -- Small helper to compute the name to use when introducing the fvar in the context
   let totalNumProps := (outputIsProp.filter (fun b => b)).size
   let mkFreshAnon isProp :=
     if isProp then mkFreshAnonPropUserName else mkFreshUserName `x
   let mkFreshName (nPropsBefore : Nat) (i : Nat) (isProp : Bool) : TacticM Name := do
-    trace[Progress] "i: {i}, isProp: {isProp}"
+    trace[Step] "i: {i}, isProp: {isProp}"
     -- Use the user-provided name if possible
     if h : i < args.ids.size then
       match args.ids[i] with
@@ -541,7 +541,7 @@ def introOutputs (args : Args) (fExpr : Expr) :
     if isProp then nPropsBefore := nPropsBefore + 1
     ids := ids.push name
 
-  trace[Progress] "ids: {ids}"
+  trace[Step] "ids: {ids}"
   let (outputIds, postsIds) := ids.toList.splitAt prefixLength
 
   -- Introduce the outputs
@@ -581,7 +581,7 @@ def introOutputs (args : Args) (fExpr : Expr) :
     - we then use the other tactic on the preconditions
  -/
 def trySolvePreconditions (args : Args) (newPropGoals : List MVarId) : TacticM (List (MVarId × OptTask (Option Expr))) := do
-  withTraceNode `Progress (fun _ => pure m!"trySolvePreconditions") do
+  withTraceNode `Step (fun _ => pure m!"trySolvePreconditions") do
   let ordPropGoals ←
     newPropGoals.mapM (fun g => do
       let ty ← g.getType
@@ -616,7 +616,7 @@ The main thing we do is simplify the post-conditions.
 TODO: simplify or remove this function.
 -/
 def postprocessMainGoal (mainGoal : Option MainGoal) : TacticM (Option MainGoal) := do
-  withTraceNode `Progress (fun _ => pure m!"postprocessMainGoal") do
+  withTraceNode `Step (fun _ => pure m!"postprocessMainGoal") do
   match mainGoal with
   | none => pure none
   | some mainGoal =>
@@ -624,8 +624,8 @@ def postprocessMainGoal (mainGoal : Option MainGoal) : TacticM (Option MainGoal)
     traceGoalWithNode "current goal"
     -- Simplify the post-conditions
     let args : Simp.SimpArgs :=
-      {simpThms := #[← progressPostSimpExt.getTheorems],
-       simprocs := #[← progressPostSimprocExt.getSimprocs] }
+      {simpThms := #[← stepPostSimpExt.getTheorems],
+       simprocs := #[← stepPostSimprocExt.getSimprocs] }
     -- Simplify
     let posts ←
       Simp.simpAt true { maxDischargeDepth := 0, failIfUnchanged := false }
@@ -634,10 +634,10 @@ def postprocessMainGoal (mainGoal : Option MainGoal) : TacticM (Option MainGoal)
     | none =>
       -- We actually closed the goal: we shouldn't get there
       -- TODO: make this more robust
-      trace[Progress] "Goal closed by simplifying the introduced post-conditions"
+      trace[Step] "Goal closed by simplifying the introduced post-conditions"
       pure none
     | some posts =>
-      trace[Progress] "Goal not closed"
+      trace[Step] "Goal not closed"
       withMainContext do
       let outputs ← posts.mapM fun fvid => do
         let name ← fvid.getUserName
@@ -651,14 +651,14 @@ def postprocessMainGoal (mainGoal : Option MainGoal) : TacticM (Option MainGoal)
       `ok ... ⦃ x₀ ... xₙ => ... ⦄`
       -/
       let r ← Simp.simpAt true { maxDischargeDepth := 1, failIfUnchanged := false}
-        {simpThms := #[← progressSimpExt.getTheorems], declsToUnfold := #[``pure]} (.targets #[] true)
+        {simpThms := #[← stepSimpExt.getTheorems], declsToUnfold := #[``pure]} (.targets #[] true)
       if r.isSome then
         pure (some ({goal := ← getMainGoal, outputs} : MainGoal))
       else pure none
 
-def progressWith (args : Args) (isLet:Bool) (fExpr : Expr) (th : Expr) :
+def stepWith (args : Args) (isLet:Bool) (fExpr : Expr) (th : Expr) :
   TacticM Goals := do
-  withTraceNode `Progress (fun _ => pure m!"progressWith") do
+  withTraceNode `Step (fun _ => pure m!"stepWith") do
   -- Attempt to instantiate the theorem and introduce it in the context
   let newGoals ← tryMatch isLet th
   --
@@ -669,12 +669,12 @@ def progressWith (args : Args) (isLet:Bool) (fExpr : Expr) (th : Expr) :
      in parallel) -/
   -- Split between the sub-goals which are propositions and the others
   let newGoals ← newGoals.filterM fun mvar => not <$> mvar.isAssigned
-  withTraceNode `Progress (fun _ => pure m!"new goals") do trace[Progress] "{newGoals}"
+  withTraceNode `Step (fun _ => pure m!"new goals") do trace[Step] "{newGoals}"
   let (newPropGoals, newNonPropGoals) ←
     newGoals.toList.partitionM fun mvar => do isProp (← mvar.getType)
-  withTraceNode `Progress (fun _ => pure m!"prop goals") do trace[Progress] "{newPropGoals}"
-  withTraceNode `Progress (fun _ => pure m!"non prop goals") do
-    trace[Progress] "{← newNonPropGoals.mapM fun mvarId => do pure ((← mvarId.getDecl).userName, mvarId)}"
+  withTraceNode `Step (fun _ => pure m!"prop goals") do trace[Step] "{newPropGoals}"
+  withTraceNode `Step (fun _ => pure m!"non prop goals") do
+    trace[Step] "{← newNonPropGoals.mapM fun mvarId => do pure ((← mvarId.getDecl).userName, mvarId)}"
   -- Attempt to solve the goals which are propositions
   let newPropGoals ← trySolvePreconditions args newPropGoals
   /- Process the main goal -/
@@ -686,9 +686,9 @@ def progressWith (args : Args) (isLet:Bool) (fExpr : Expr) (th : Expr) :
       We also simplify the goal again (to simplify let-bindings, etc.) -/
   let mainGoal ← postprocessMainGoal mainGoal
   if let some mainGoal := mainGoal then
-    withTraceNode `Progress
+    withTraceNode `Step
       (fun _ => pure m!"Main goal after simplifying the post-conditions and the target") do
-      trace[Progress] "{mainGoal.goal}"
+      trace[Step] "{mainGoal.goal}"
   /- Put everything together -/
   let newNonPropGoals ← newNonPropGoals.filterM fun mvar => not <$> mvar.isAssigned
   pure ({ unassignedVars := newNonPropGoals.toArray, preconditions := newPropGoals.toArray, mainGoal })
@@ -714,42 +714,42 @@ def tryApply (args : Args) (isLet:Bool) (fExpr : Expr) (kind : String) (th : Opt
   let res ← do
     match th with
     | none =>
-      trace[Progress] "Could not find a {kind}"
+      trace[Step] "Could not find a {kind}"
       pure none
     | some th => do
-      trace[Progress] "Lookuped up {kind}: {th}"
+      trace[Step] "Lookuped up {kind}: {th}"
       -- Apply the theorem
       let res ← do
         try
-          let res ← progressWith args isLet fExpr th
+          let res ← stepWith args isLet fExpr th
           pure (some res)
         catch _ => pure none
   match res with
   | some res => pure (some res)
   | none => pure none
 
-/-- Try to progress with an assumption.
+/-- Try to step with an assumption.
     Return `some` if we succeed, `none` otherwise.
 
     -- TODO: check that they are "compatible" with the goal to avoid a potentially expensive unification
 -/
 def tryAssumptions (args : Args) (isLet:Bool) (fExpr : Expr) :
   TacticM (Option (Goals × UsedTheorem)) := do
-  withTraceNode `Progress (fun _ => pure m!"tryAssumptions") do run
+  withTraceNode `Step (fun _ => pure m!"tryAssumptions") do run
 where
   run :=
   withMainContext do
   let ctx ← Lean.MonadLCtx.getLCtx
   let decls ← ctx.getAssumptions
   for decl in decls.reverse do
-    trace[Progress] "Trying assumption: {decl.userName} : {decl.type}"
+    trace[Step] "Trying assumption: {decl.userName} : {decl.type}"
     try
-      let goal ← progressWith args isLet fExpr decl.toExpr
+      let goal ← stepWith args isLet fExpr decl.toExpr
       return (some (goal, .localHyp decl))
     catch _ => continue
   pure none
 
-def progressAsmsOrLookupTheorem (args : Args) (withTh : Option Expr) :
+def stepAsmsOrLookupTheorem (args : Args) (withTh : Option Expr) :
   TacticM (Goals × UsedTheorem) := do
   withMainContext do
   -- Retrieve the goal
@@ -758,9 +758,9 @@ def progressAsmsOrLookupTheorem (args : Args) (withTh : Option Expr) :
   /- There might be uninstantiated meta-variables in the goal that we need
      to instantiate (otherwise we will get stuck). -/
   let goalTy ← instantiateMVars goalTy
-  trace[Progress] "progressAsmsOrLookupTheorem: target: {goalTy}"
+  trace[Step] "stepAsmsOrLookupTheorem: target: {goalTy}"
   /- Dive into the goal to lookup the theorem
-     Remark: if we don't isolate the call to `withProgressSpec` to immediately "close"
+     Remark: if we don't isolate the call to `withStepSpec` to immediately "close"
      the terms immediately, we may end up with the error:
      "(kernel) declaration has free variables"
      I'm not sure I understand why.
@@ -768,13 +768,13 @@ def progressAsmsOrLookupTheorem (args : Args) (withTh : Option Expr) :
      If such variables appear, we should just fail because the goal doesn't
      have the proper shape. -/
   let (goalIsLet, fExpr) ← do
-    withTraceNode `Progress (fun _ => pure m!"Calling getFirstBind to deconstruct the target") do
+    withTraceNode `Step (fun _ => pure m!"Calling getFirstBind to deconstruct the target") do
     getFirstBind goalTy
   /- If the user provided a theorem/assumption: use it.
      Otherwise, lookup one. -/
   match withTh with
   | some th => do
-    let goals ← progressWith args goalIsLet fExpr th
+    let goals ← stepWith args goalIsLet fExpr th
     return (goals, .givenExpr th)
   | none =>
     -- Try all the assumptions one by one and if it fails try to lookup a theorem.
@@ -785,27 +785,27 @@ def progressAsmsOrLookupTheorem (args : Args) (withTh : Option Expr) :
       fExpr.consumeMData.withApp fun mf _ => do
       pure mf.isConst
     if ¬ fIsConst then
-      trace[Progress] "Progress failed: the target function is not a constant"
-      throwError "Progress failed"
+      trace[Step] "Step failed: the target function is not a constant"
+      throwError "Step failed"
     else do
-      trace[Progress] "No assumption succeeded: trying to lookup a pspec theorem"
+      trace[Step] "No assumption succeeded: trying to lookup a pspec theorem"
       let pspecs : Array Name ← do
-        let thNames ← progressAttr.find? fExpr
+        let thNames ← stepAttr.find? fExpr
         /- TODO: because of reduction, there may be several valid theorems (for
            instance for the scalars). We need to sort them from most specific to
            least specific. For now, we assume the most specific theorems are at
            the end. -/
         let thNames := thNames.reverse
-        trace[Progress] "Looked up pspec theorems: {thNames}"
+        trace[Step] "Looked up pspec theorems: {thNames}"
         pure thNames
       -- Try the theorems one by one
       for pspec in pspecs do
         let pspecExpr ← Term.mkConst pspec
         match ← tryApply args goalIsLet fExpr "pspec theorem" pspecExpr with
-        | some goals => return (goals, .progressThm pspec)
+        | some goals => return (goals, .stepThm pspec)
         | none => pure ()
       -- It failed: try to use the recursive assumptions
-      trace[Progress] "Failed using a pspec theorem: trying to use a recursive assumption"
+      trace[Step] "Failed using a pspec theorem: trying to use a recursive assumption"
       -- We try to apply the assumptions of kind "auxDecl"
       -- TODO: check that they are "compatible" with the goal to avoid a potentially expensive unification
       let ctx ← Lean.MonadLCtx.getLCtx
@@ -814,46 +814,46 @@ def progressAsmsOrLookupTheorem (args : Args) (withTh : Option Expr) :
         | .default | .implDetail => false | .auxDecl => true)
       -- TODO: introduce a helper for this
       for decl in decls.reverse do
-        trace[Progress] "Trying recursive assumption: {decl.userName} : {decl.type}"
+        trace[Step] "Trying recursive assumption: {decl.userName} : {decl.type}"
         try
-          let goals ← progressWith args goalIsLet fExpr decl.toExpr
+          let goals ← stepWith args goalIsLet fExpr decl.toExpr
           return (goals, .localHyp decl)
         catch _ => continue
       -- Nothing worked: failed
-      let msg := "Progress failed: could not find a local assumption or a theorem to apply"
-      trace[Progress] msg
+      let msg := "Step failed: could not find a local assumption or a theorem to apply"
+      trace[Step] msg
       throwError msg
 
-syntax progressArgs := Parser.Tactic.optConfig ("with" term)? ("as" " ⟨ " binderIdent,* " ⟩")? ("by" tacticSeq)?
+syntax stepArgs := Parser.Tactic.optConfig ("with" term)? ("as" " ⟨ " binderIdent,* " ⟩")? ("by" tacticSeq)?
 
-def parseProgressArgs
-: TSyntax ``Aeneas.Progress.progressArgs →
+def parseStepArgs
+: TSyntax ``Aeneas.Step.stepArgs →
   TacticM (Config × Option Expr × Array (Option Name) × Bool × Option Name × Option Syntax.Tactic)
-| args@`(progressArgs| $config $[with $pspec:term]? $[as ⟨ $ids,* ⟩]? $[by $byTac]? ) =>
+| args@`(stepArgs| $config $[with $pspec:term]? $[as ⟨ $ids,* ⟩]? $[by $byTac]? ) =>
   withMainContext do
-  withTraceNode `Progress (fun _ => do pure m!"progressArgs") do
-  trace[Progress] "Progress arguments: {args.raw}"
+  withTraceNode `Step (fun _ => do pure m!"stepArgs") do
+  trace[Step] "Step arguments: {args.raw}"
   let config ← elabPartialConfig config
-  trace[Progress] "config: {repr config}"
+  trace[Step] "config: {repr config}"
   let withTh?: Option Expr ← Option.sequence <| pspec.map fun
     /- We have to make a case disjunction, because if we treat identifiers like
        terms, then Lean will not succeed in infering their implicit parameters
-       (`progress` does that by matching against the goal). -/
+       (`step` does that by matching against the goal). -/
     | `($stx:ident) => do
       match (← getLCtx).findFromUserName? stx.getId with
       | .some decl =>
-        trace[Progress] "With arg (local decl): {stx.raw}"
+        trace[Step] "With arg (local decl): {stx.raw}"
         return decl.toExpr
       | .none =>
         -- Not a local declaration: should be a theorem
-        trace[Progress] "With arg (theorem): {stx.raw}"
+        trace[Step] "With arg (theorem): {stx.raw}"
         let some e ← Term.resolveId? stx (withInfo := true)
           | throwError m!"Could not find theorem: {pspec}"
         return e
     | term => do
-      trace[Progress] "With arg (term): {term}"
+      trace[Step] "With arg (term): {term}"
       Tactic.elabTerm term none
-  if let .some pspec := withTh? then trace[Progress] "With arg: elaborated expression {pspec}"
+  if let .some pspec := withTh? then trace[Step] "With arg: elaborated expression {pspec}"
   let userGaveIds := ids.isSome
   let ids := ids.getD ∅
     |>.getElems.map fun
@@ -864,7 +864,7 @@ def parseProgressArgs
       let (ids, postsBasename) ← getVarNamesFromGoal
       pure (ids, false, postsBasename)
     else pure (ids, true, none)
-  trace[Progress] "User-provided ids: {ids}"
+  trace[Step] "User-provided ids: {ids}"
   let byTac : Option Syntax.Tactic := match byTac with
     | none => none
     | some byTac => some ⟨byTac.raw⟩
@@ -873,37 +873,37 @@ def parseProgressArgs
 
 /-- Use `agrind` after preprocessing goal the goal, in particular to simplify arithmetic expressions. -/
 def evalAGrindWithPreprocess (withGroundSimprocs : Bool) (config : Grind.Config) : TacticM Unit := do
-  withTraceNode `Progress (fun _ => do pure m!"evalAGrindWithPreprocess") do
+  withTraceNode `Step (fun _ => do pure m!"evalAGrindWithPreprocess") do
   traceGoalWithNode "before preprocessing"
   let simpArgs : Simp.SimpArgs ← ScalarTac.getSimpArgs
   let sconfig : Simp.Config := {dsimp := false, failIfUnchanged := false, maxDischargeDepth := 1}
   match ← ScalarTac.simpAsmsTarget true sconfig simpArgs with
   | none =>
-    trace[Progress] "Goal solved by preprocessing!"
+    trace[Step] "Goal solved by preprocessing!"
   | some _ =>
     traceGoalWithNode "after preprocessing"
     /- We reduce the search space but increase the number of instances (we need this when the
        context is big).
 
        TODO: an issue is that `omega` used to split all disjunctions.
-       TODO: make those options of `progress`
+       TODO: make those options of `step`
        TODO: fine tune the parameters
      -/
     let params ← Aeneas.Grind.mkParams config #[Aeneas.Grind.agrindExt.getState (← Lean.getEnv)] withGroundSimprocs
     let mvarId ← Lean.Elab.Tactic.getMainGoal
     try
       Aeneas.Grind.agrindEval config params mvarId
-    catch e => trace[Progress] "Grind failed:\n{e.toMessageData}"
+    catch e => trace[Step] "Grind failed:\n{e.toMessageData}"
 
-def evalProgressCore (config : Config) (keepPretty : Option Name) (withArg : Option Expr)
+def evalStepCore (config : Config) (keepPretty : Option Name) (withArg : Option Expr)
   (ids : Array (Option Name)) (idsUserProvided : Bool) (postsBasename : Option Name := none)
   (byTacStx : Option Syntax.Tactic)
   : TacticM Stats := do
-  withTraceNode `Progress (fun _ => pure m!"evalProgress") do
+  withTraceNode `Step (fun _ => pure m!"evalStep") do
   /- Simplify the goal -- TODO: this might close it: we need to check that and abort if necessary,
      and properly track that in the `Stats` -/
   let _ ← Simp.simpAt true { maxDischargeDepth := 1, failIfUnchanged := false}
-      {simpThms := #[← progressSimpExt.getTheorems]} (.targets #[] true)
+      {simpThms := #[← stepSimpExt.getTheorems]} (.targets #[] true)
   withMainContext do
 
   /- **Assumption tactic**:
@@ -918,7 +918,7 @@ def evalProgressCore (config : Config) (keepPretty : Option Name) (withArg : Opt
       /- Preprocessing step for `singleAssumptionTac` -/
       let singleAssumptionTacDtree ← singleAssumptionTacPreprocess
       pure (some do
-        withTraceNode `Progress (fun _ => pure m!"Attempting to solve with `singleAssumptionTac`") do
+        withTraceNode `Step (fun _ => pure m!"Attempting to solve with `singleAssumptionTac`") do
         singleAssumptionTacCore singleAssumptionTacDtree (instMVars := config.inferGhostVars))
     else pure none
 
@@ -932,7 +932,7 @@ def evalProgressCore (config : Config) (keepPretty : Option Name) (withArg : Opt
     There is a fast track: if the goal is not an arithmetic goal, we skip
     (note that otherwise, `scalarTac` would try to prove a contradiction) -/
   let scalarTac : TacticM Unit := do
-    withTraceNode `Progress (fun _ => pure m!"Attempting to solve with `scalarTac`") do
+    withTraceNode `Step (fun _ => pure m!"Attempting to solve with `scalarTac`") do
     if ← ScalarTac.goalIsLinearInt then
       /- Also: we don't try to split the goal if it is a conjunction
          (it shouldn't be), but we split the disjunctions. -/
@@ -946,7 +946,7 @@ def evalProgressCore (config : Config) (keepPretty : Option Name) (withArg : Opt
   let localAsms ← pure ((← (← getLCtx).getAssumptions).map LocalDecl.fvarId)
   let simpArgs : Simp.SimpArgs := {simpThms := #[simpLemmas], hypsToUse := localAsms.toArray}
   let simpTac : TacticM Unit := do
-    withTraceNode `Progress (fun _ => pure m!"Attempting to solve with `simp [*]`") do
+    withTraceNode `Step (fun _ => pure m!"Attempting to solve with `simp [*]`") do
     -- Simplify the goal
     let r ← Simp.simpAt false { maxDischargeDepth := 1 } simpArgs (.targets #[] true)
     -- Raise an error if the goal is not proved
@@ -959,7 +959,7 @@ def evalProgressCore (config : Config) (keepPretty : Option Name) (withArg : Opt
   let byTac := match byTacStx with
     | none => []
     | some tacticCode => [
-      withTraceNode `Progress (fun _ => pure m!"Attempting to solve with the user tactic: `{byTacStx}`") do
+      withTraceNode `Step (fun _ => pure m!"Attempting to solve with the user tactic: `{byTacStx}`") do
       /- It may happen that the tactic introduces auxiliary theorems to hide some proofs details: because
          the environment containing those proofs will get discarded, we need to inline them -/
       let g ← getMainGoal
@@ -975,30 +975,30 @@ def evalProgressCore (config : Config) (keepPretty : Option Name) (withArg : Opt
   let allTacs := simpTac ++ grindTac ++ scalarTac ++ byTac
   let solvePreconditionTac :=
     withMainContext do
-    withTraceNode `Progress (fun _ => pure m!"Trying to solve a precondition") do
-    trace[Progress] "Precondition: {← getMainGoal}"
+    withTraceNode `Step (fun _ => pure m!"Trying to solve a precondition") do
+    trace[Step] "Precondition: {← getMainGoal}"
     try
       firstTacSolve allTacs
-      trace[Progress] "Precondition solved!"
+      trace[Step] "Precondition solved!"
     catch _ =>
-      trace[Progress] "Precondition not solved"
+      trace[Step] "Precondition not solved"
   let args : Args := {
     async := config.async,
     inferGhostVars := config.inferGhostVars,
     keepPretty, ids, idsUserProvided, postsBasename, assumTac := customAssumTac,
     solvePreconditionTac, byTacSyntax := byTacStx
   }
-  let (goals, usedTheorem) ← progressAsmsOrLookupTheorem args withArg
-  trace[Progress] "Progress done"
+  let (goals, usedTheorem) ← stepAsmsOrLookupTheorem args withArg
+  trace[Step] "Step done"
   return ⟨ goals, usedTheorem ⟩
 
-def evalProgress
+def evalStep
   (config : Config) (keepPretty : Option Name) (withArg: Option Expr)
   (ids: Array (Option Name)) (idsUserProvided : Bool)
   (postsBasename : Option Name := none) (byTac : Option Syntax.Tactic)
   : TacticM UsedTheorem := do
   focus do
-  let ⟨goals, usedTheorem⟩ ← evalProgressCore config keepPretty withArg ids idsUserProvided postsBasename byTac
+  let ⟨goals, usedTheorem⟩ ← evalStepCore config keepPretty withArg ids idsUserProvided postsBasename byTac
   -- Wait for all the proof attempts to finish
   let mut sgs := #[]
   for (mvarId, proof) in goals.preconditions do
@@ -1015,11 +1015,11 @@ def evalProgress
   setGoals (goals.unassignedVars.toList ++ sgs.toList ++ mainGoal)
   pure usedTheorem
 
-/-- The `progress` tactic is used to reason about monadic goals.
+/-- The `step` tactic is used to reason about monadic goals.
 It is a bit equivalent to the `mvcgen` tactic from the Lean standard library.
 
-The `progress`tactic works by looking for a suitable theorem (either provided by the user
-or looked up in the database of `progress` theorems) which describes the behavior of a monadic
+The `step`tactic works by looking for a suitable theorem (either provided by the user
+or looked up in the database of `step` theorems) which describes the behavior of a monadic
 function, then applying it to the current goal. It then introduces the
 existentially quantified variables and splits the conjunctions in the
 post-condition, before trying to solve the preconditions.
@@ -1031,7 +1031,7 @@ h : 2 * (a.val + 1) < U32.max
   let b ← a + 1#u32
   2 * b) ⦃ c => c > 0 ⦄
 ```
-`progress as ⟨ b ⟩` will lookup the theorem:
+`step as ⟨ b ⟩` will lookup the theorem:
 ```lean
 theorem UScalar.add_spec (x y : UScalar ty) (h : x.val + y.val < UScalar.max ty) :
   UScalar.add x y ⦃ z => z.val = x.val + y.val ⦄
@@ -1048,9 +1048,9 @@ h_b : b.val = a.val + 1
 ⊢ 2 * b ⦃ c => c > 0 ⦄
 ```
 
-Note that `progress` is able to use the current theorem when doing recursive proofs.
+Note that `step` is able to use the current theorem when doing recursive proofs.
 
-*Remark:** `progress` actually also introduces a dummy variable in the context,
+*Remark:** `step` actually also introduces a dummy variable in the context,
 which is pretty printed to display information to the user. For instance, in the
 goal above we actually insert a variable `_ : [> b ← a + 1#u32 <]` so that the user keeps
 track of the origin of `b`.
@@ -1066,22 +1066,22 @@ The user can provide several optional arguments:
   variables/conditions than names provided by the user, fresh names are generated.
   If there are more names than variables/conditions, a warning is displayed.
 - `by <tactic>`: use the given tactic to solve the preconditions.
-- `progress?`: displays the name of the theorem/assumption used.
-- `progress` has various other options to, for instance, tweak the calls to `grind`.
-  The syntax is, e.g.: `progress +splitIte (splits := 6)`.
-  See `Aeneas.Progress.Config` for the full set of options.
+- `step?`: displays the name of the theorem/assumption used.
+- `step` has various other options to, for instance, tweak the calls to `grind`.
+  The syntax is, e.g.: `step +splitIte (splits := 6)`.
+  See `Aeneas.Step.Config` for the full set of options.
 
-**`progress?`**: displays the name of the theorem used.
+**`step?`**: displays the name of the theorem used.
 
 **Alternative syntax:**
-The `progress` tactic also supports the following syntax:
+The `step` tactic also supports the following syntax:
 `let ⟨ id1, id2, ... ⟩ ←[+splitIte (splits := 6)]? <withArg> (by <tactic>)?`
 which is equivalent to:
-`progress +splitIte (splits := 6) with <withArg> as ⟨ id1, id2, ... ⟩ by <tactic>`
+`step +splitIte (splits := 6) with <withArg> as ⟨ id1, id2, ... ⟩ by <tactic>`
 
-**The `progress` attribute:**
-To make a theorem available for `progress`, the user can tag it with the
-`@[progress]` attribute. The theorem must have the following shape:
+**The `step` attribute:**
+To make a theorem available for `step`, the user can tag it with the
+`@[step]` attribute. The theorem must have the following shape:
 ```lean
 theorem thm_name (arg1 : ty1) ... (argn : tyn)
     (h_pre1 : precondition_1) ... (h_prem : precondition_m) :
@@ -1090,7 +1090,7 @@ theorem thm_name (arg1 : ty1) ... (argn : tyn)
 where `f` is a monadic function with type `Result ...`.
 
 **Ghost Variables:**
-It is possible to write progress theorems which use ghost variables, i.e., variables
+It is possible to write step theorems which use ghost variables, i.e., variables
 which do not appear as an input of the monadic function. For instance, in the theorem
 below, `map` is a ghost variable as it does not appear in the arguments of `hashmap_insert`.
 ```lean
@@ -1100,69 +1100,69 @@ theorem hashmap_insert_spec {k v : Type} [BEq k] [Hashable k]
     HashMap.insert hmap key val ⦃ (newMap : HashMap k v) =>
     ... ⦄
 ```
-When encoutering ghost variables, `progress` will try to instantiate them by looking
+When encoutering ghost variables, `step` will try to instantiate them by looking
 for local assumptions which match the theorem assumptions, using heuristics to find
 the best instantiation when several are possible.
 
-**Progress\*:**
-When the user wants to make progress by several step, they can use the `progress*` tactic,
-which repeatedly calls `progress` until no further progress can be made. See the documentation
-of `progress*` for more details.
+**Step\*:**
+When the user wants to make progress by several step, they can use the `step*` tactic,
+which repeatedly calls `step` until no further progress can be made. See the documentation
+of `step*` for more details.
 -/
-elab (name := progress) "progress" args:progressArgs : tactic => do
-  let (config, withArg, ids, idsUserProvided, postsBasename, byTac) ← parseProgressArgs args
-  evalProgress config none withArg ids idsUserProvided postsBasename byTac *> return ()
+elab (name := step) "step" args:stepArgs : tactic => do
+  let (config, withArg, ids, idsUserProvided, postsBasename, byTac) ← parseStepArgs args
+  evalStep config none withArg ids idsUserProvided postsBasename byTac *> return ()
 
-@[inherit_doc progress]
-elab tk:"progress?" args:progressArgs : tactic => do
-  let (config, withArg, ids, idsUserProvided, postsBasename, byTac) ← parseProgressArgs args
-  let stats ← evalProgress config none withArg ids idsUserProvided postsBasename byTac
+@[inherit_doc step]
+elab tk:"step?" args:stepArgs : tactic => do
+  let (config, withArg, ids, idsUserProvided, postsBasename, byTac) ← parseStepArgs args
+  let stats ← evalStep config none withArg ids idsUserProvided postsBasename byTac
   let mut stxArgs := args.raw
   -- Update the syntax to add the `with thm`
   if stxArgs[1].isNone then
     let withArg := mkNullNode #[mkAtom "with", ← stats.toSyntax]
     stxArgs := stxArgs.setArg 1 withArg
-  let tac := mkNode `Aeneas.Progress.progress #[mkAtom "progress", stxArgs]
+  let tac := mkNode `Aeneas.Step.step #[mkAtom "step", stxArgs]
   let fmt ← PrettyPrinter.ppCategory ``Lean.Parser.Tactic.tacticSeq tac
   Meta.Tactic.TryThis.addSuggestion tk fmt.pretty (origSpan? := ← getRef)
 
 syntax optConfig := Parser.Tactic.optConfig
 
-@[inherit_doc progress]
-syntax (name := letProgress) "let" noWs "*" " ⟨ " binderIdent,* " ⟩" colGe
+@[inherit_doc step]
+syntax (name := letStep) "let" noWs "*" " ⟨ " binderIdent,* " ⟩" colGe
   " ← " colGe ("[" Parser.Tactic.optConfig " ] ")? ("*?" <|> "*" <|> term) ("by" tacticSeq)? : tactic
 
-def parseLetProgress
-: TSyntax ``Aeneas.Progress.letProgress ->
+def parseLetStep
+: TSyntax ``Aeneas.Step.letStep ->
   TacticM (Config × Option Expr × Bool × Array (Option Name) × Option Name × Option Syntax.Tactic)
 | args@`(tactic| let* ⟨ $ids,* ⟩ ← $[[$config]]? $pspec $[by $byTac]?) =>  withMainContext do
-  trace[Progress] "Progress arguments: {args.raw}"
+  trace[Step] "Step arguments: {args.raw}"
   let ((withThm, suggest) : (Option Expr × Bool)) ← do
     /- We have to make a case disjunction, because if we treat identifiers like
       terms, then Lean will not succeed in infering their implicit parameters
-      (`progress` does that by matching against the goal). -/
+      (`step` does that by matching against the goal). -/
     match pspec with
     | `($stx:ident) => do
       match (← getLCtx).findFromUserName? stx.getId with
       | .some decl =>
-        trace[Progress] "With arg (local decl): {stx.raw}"
+        trace[Step] "With arg (local decl): {stx.raw}"
         pure (some decl.toExpr, false)
       | .none =>
         -- Not a local declaration: should be a theorem
-        trace[Progress] "With arg (theorem): {stx.raw}"
+        trace[Step] "With arg (theorem): {stx.raw}"
         let some e ← Term.resolveId? stx (withInfo := true)
           | throwError m!"Could not find theorem: {pspec}"
         pure (some e, false)
     | term => do
-      trace[Progress] "term.raw.getKind: {term.raw.getKind}"
+      trace[Step] "term.raw.getKind: {term.raw.getKind}"
       if term.raw.getKind = `token.«*» then
-        trace[Progress] "With arg: *"
+        trace[Step] "With arg: *"
         pure (none, false)
       else if term.raw.getKind = `token.«*?» then
-        trace[Progress] "With arg: ?"
+        trace[Step] "With arg: ?"
         pure (none, true)
       else
-        trace[Progress] "With arg (term): {term}"
+        trace[Step] "With arg (term): {term}"
         pure (some (← Tactic.elabTerm term none), false)
   let numIds := ids.getElems.size
   let ids := ids.getElems.map fun
@@ -1177,38 +1177,38 @@ def parseLetProgress
   let byTac : Option Syntax.Tactic := match byTac with
     | none => none
     | some byTac => some ⟨byTac.raw⟩
-  trace[Progress] "User-provided ids: {ids}"
+  trace[Step] "User-provided ids: {ids}"
   return (config, withThm, suggest, ids, postsBasename, byTac)
 | _ => throwUnsupportedSyntax
 
-elab tk:letProgress : tactic => do
+elab tk:letStep : tactic => do
   withMainContext do
-  let (config, withArg, suggest, ids, postsBasename, byTac) ← parseLetProgress tk
+  let (config, withArg, suggest, ids, postsBasename, byTac) ← parseLetStep tk
   let idsUserProvided := true
-  let stats ← evalProgress config (some (.str .anonymous "_")) withArg ids idsUserProvided postsBasename byTac
+  let stats ← evalStep config (some (.str .anonymous "_")) withArg ids idsUserProvided postsBasename byTac
   let mut stxArgs := tk.raw
   if suggest then
-    trace[Progress] "suggest is true"
+    trace[Step] "suggest is true"
     let withArg ← stats.toSyntax
     stxArgs := stxArgs.setArg 7 withArg
-    let stxArgs' : TSyntax `Aeneas.Progress.letProgress := ⟨ stxArgs ⟩
-    trace[Progress] "stxArgs': {stxArgs}"
+    let stxArgs' : TSyntax `Aeneas.Step.letStep := ⟨ stxArgs ⟩
+    trace[Step] "stxArgs': {stxArgs}"
     Meta.Tactic.TryThis.addSuggestion tk stxArgs' (origSpan? := ← getRef)
 
 namespace Test
   open Std Result
 
   -- Show the traces:
-  -- set_option trace.Progress true
+  -- set_option trace.Step true
   -- set_option pp.rawOnError true
 
   set_option says.verify true
 
   -- The following command displays the database of theorems:
-  -- #eval showStoredProgressThms
+  -- #eval showStoredStepThms
   open alloc.vec
 
-  /- This test case checks what happens when `progress`:
+  /- This test case checks what happens when `step`:
      - manages to solve the current goal
      - but doesn't solve some preconditions
      At some point there was a bug with the goal management.
@@ -1223,11 +1223,11 @@ x y : UScalar ty
   #guard_msgs in
   example {ty} {x y : UScalar ty} :
     x + y ⦃ _ => True ⦄ := by
-    progress as ⟨ z, h1 ⟩
+    step as ⟨ z, h1 ⟩
 
   example {ty} {x y : UScalar ty} (h : x.val + y.val ≤ UScalar.max ty) :
     x + y ⦃ _ => True ⦄ := by
-    progress as ⟨ z, h1 ⟩
+    step as ⟨ z, h1 ⟩
 
   example {ty} {x y : UScalar ty} (h : x.val + y.val ≤ UScalar.max ty) :
     x + y ⦃ _ => True ⦄ := by
@@ -1254,8 +1254,8 @@ _✝ : z1 = y + 2
     (do
       let (y, _) ← addToPair x
       addToPair y) ⦃ y _ => y = x + 2 ⦄ := by
-    progress with addToPair_spec as ⟨ y, z, h ⟩
-    progress with addToPair_spec as ⟨ y1, z1, h1 ⟩
+    step with addToPair_spec as ⟨ y, z, h ⟩
+    step with addToPair_spec as ⟨ y1, z1, h1 ⟩
 
   /--
   info: Try this:
@@ -1316,66 +1316,66 @@ info: example
     (do
       let z1 ← x + y
       z1 + x) ⦃ z => z.val = 2 * x.val + y.val ⦄ := by
-    progress with UScalar.add_spec as ⟨ z1, h1 ⟩
-    progress with UScalar.add_spec as ⟨ z2, h2 ⟩
+    step with UScalar.add_spec as ⟨ z1, h1 ⟩
+    step with UScalar.add_spec as ⟨ z2, h2 ⟩
     scalar_tac
 
   example {ty} {x y : UScalar ty}
     (hmax : x.val + y.val ≤ UScalar.max ty) :
     x + y ⦃ z => z.val = x.val + y.val ⦄ := by
-    progress as ⟨ z, h1 ⟩
+    step as ⟨ z, h1 ⟩
     scalar_tac
 
   example {ty} {x y : IScalar ty}
     (hmin : IScalar.min ty ≤ x.val + y.val)
     (hmax : x.val + y.val ≤ IScalar.max ty) :
     x + y ⦃ z => z.val = x.val + y.val ⦄ := by
-    progress as ⟨ z, h1 ⟩
+    step as ⟨ z, h1 ⟩
     scalar_tac
 
   example {ty} {x y : UScalar ty}
     (hmax : x.val + y.val ≤ UScalar.max ty) :
     x + y ⦃ z => z.val = x.val + y.val ⦄ := by
-    progress? as ⟨ z, h1 ⟩ says progress with UScalar.add_spec as ⟨ z, h1 ⟩
+    step? as ⟨ z, h1 ⟩ says step with UScalar.add_spec as ⟨ z, h1 ⟩
     scalar_tac
 
   example {ty} {x y : IScalar ty}
     (hmin : IScalar.min ty ≤ x.val + y.val)
     (hmax : x.val + y.val ≤ IScalar.max ty) :
     x + y ⦃ z => z.val = x.val + y.val ⦄ := by
-    progress? as ⟨ z, h1 ⟩ says progress with IScalar.add_spec as ⟨ z, h1 ⟩
+    step? as ⟨ z, h1 ⟩ says step with IScalar.add_spec as ⟨ z, h1 ⟩
     scalar_tac
 
   example {ty} {x y : UScalar ty}
     (hmax : x.val + y.val ≤ UScalar.max ty) :
     x + y ⦃ z => z.val = x.val + y.val ⦄ := by
-    progress with UScalar.add_spec as ⟨ z ⟩
+    step with UScalar.add_spec as ⟨ z ⟩
     scalar_tac
 
   example {ty} {x y : IScalar ty}
     (hmin : IScalar.min ty ≤ x.val + y.val)
     (hmax : x.val + y.val ≤ IScalar.max ty) :
     x + y ⦃ z => z.val = x.val + y.val ⦄ := by
-    progress with IScalar.add_spec as ⟨ z ⟩
+    step with IScalar.add_spec as ⟨ z ⟩
     scalar_tac
 
   example {x y : U32}
     (hmax : x.val + y.val ≤ U32.max) :
     x + y ⦃ z => z.val = x.val + y.val ⦄ := by
     -- This spec theorem is suboptimal (compared to `U32.add_spec`), but it is good to check that it works
-    progress with UScalar.add_spec as ⟨ z, h1 ⟩
+    step with UScalar.add_spec as ⟨ z, h1 ⟩
     scalar_tac
 
   example {x y : U32}
     (hmax : x.val + y.val ≤ U32.max) :
     x + y ⦃ z => z.val = x.val + y.val ⦄ := by
-    progress with U32.add_spec as ⟨ z, h1 ⟩
+    step with U32.add_spec as ⟨ z, h1 ⟩
     scalar_tac
 
   example {x y : U32}
     (hmax : x.val + y.val ≤ U32.max) :
     x + y ⦃ z => z.val = x.val + y.val ⦄ := by
-    progress as ⟨ z, h1 ⟩
+    step as ⟨ z, h1 ⟩
     scalar_tac
 
   /- Checking that universe instantiation works: the original spec uses
@@ -1383,16 +1383,16 @@ info: example
   example {α : Type} (v: Vec α) (i: Usize) (x : α)
     (hbounds : i.val < v.length) :
     v.update i x ⦃ nv => nv.val = v.val.set i.val x ⦄ := by
-    progress
+    step
     simp [*]
 
   example {α : Type} (v: Vec α) (i: Usize) (x : α)
     (hbounds : i.val < v.length) :
     v.update i x ⦃ nv => nv.val = v.val.set i.val x ⦄ := by
-    progress? says progress with Vec.update_spec
+    step? says step with Vec.update_spec
     simp [*]
 
-  /- Checking that progress can handle nested blocks -/
+  /- Checking that step can handle nested blocks -/
   example {α : Type} (v: Vec α) (i: Usize) (x : α)
     (hbounds : i.val < v.length) :
     (do
@@ -1401,7 +1401,7 @@ info: example
           .ok ())
         .ok ()) ⦃ _ => True ⦄
       := by
-    progress
+    step
 
   /- Checking the case where simplifying the goal after instantiating the
      pspec theorem actually solves it, and where the function is not a constant.
@@ -1409,20 +1409,20 @@ info: example
   example {x : U32}
     (f : U32 → Std.Result Unit) (h : ∀ x, f x ⦃ _ => True ⦄) :
     f x ⦃ _ => True ⦄ := by
-    progress
+    step
 
   example {x : U32}
     (f : U32 → Std.Result Unit) (h : ∀ x, f x ⦃ _ => True ⦄) :
     f x ⦃ _ => True ⦄ := by
-    progress? says progress with h
+    step? says step with h
 
   /- The use of `right` introduces a meta-variable in the goal, that we
-     need to instantiate (otherwise `progress` gets stuck) -/
+     need to instantiate (otherwise `step` gets stuck) -/
   example {ty} {x y : UScalar ty}
     (hmax : x.val + y.val ≤ UScalar.max ty) :
     False ∨ x + y ⦃ z => z.val = x.val + y.val ⦄ := by
     right
-    progress as ⟨ z, h1 ⟩
+    step as ⟨ z, h1 ⟩
     scalar_tac
 
   example {ty} {x y : IScalar ty}
@@ -1430,7 +1430,7 @@ info: example
     (hmax : x.val + y.val ≤ IScalar.max ty) :
     False ∨ x + y ⦃ z => z.val = x.val + y.val ⦄ := by
     right
-    progress? as ⟨ z, h1 ⟩ says progress with IScalar.add_spec as ⟨ z, h1 ⟩
+    step? as ⟨ z, h1 ⟩ says step with IScalar.add_spec as ⟨ z, h1 ⟩
     scalar_tac
 
   /--
@@ -1450,7 +1450,7 @@ hf : ∀ (x y : U32), ↑x < 10 → ↑y < 10 → f x y ⦃ x✝ => True ⦄
   #guard_msgs in
   example {x y} (f : U32 → U32 → Result U32) (hf : ∀ x y, x.val < 10 → y.val < 10 → f x y ⦃ _ => True⦄) :
     f x y ⦃ _ => True⦄ := by
-    progress
+    step
 
   -- Testing with mutually recursive definitions
   mutual
@@ -1478,35 +1478,35 @@ hf : ∀ (x y : U32), ↑x < 10 → ↑y < 10 → f x y ⦃ x✝ => True ⦄
 
   section
     mutual
-      @[local progress]
+      @[local step]
       theorem Tree.size_spec (t : Tree) :
         t.size ⦃ i => i ≥ 0 ⦄ := by
         cases h: t -- TODO: `cases t` doesn't work
         simp [Tree.size]
-        progress
+        step
         scalar_tac
 
-      @[local progress]
+      @[local step]
       theorem Trees.size_spec (t : Trees) :
         t.size ⦃ i => i ≥ 0 ⦄ := by
         cases h: t <;> simp [Trees.size] -- TODO: `cases t` doesn't work
-        progress
-        progress? says progress with Trees.size_spec
+        step
+        step? says step with Trees.size_spec
         scalar_tac
     end
   end
 
-  -- Testing progress on theorems containing local let-bindings
+  -- Testing step on theorems containing local let-bindings
   def add (x y : U32) : Std.Result U32 := x + y
 
   section
-    /- Testing progress on theorems containing local let-bindings as well as
+    /- Testing step on theorems containing local let-bindings as well as
        the `local` attribute kind -/
-    @[local progress] theorem add_spec' (x y : U32) (h : x.val + y.val ≤ U32.max) :
+    @[local step] theorem add_spec' (x y : U32) (h : x.val + y.val ≤ U32.max) :
       let tot := x.val + y.val
       x + y ⦃ z => z.val = tot ⦄ := by
       simp
-      progress with U32.add_spec
+      step with U32.add_spec
       scalar_tac
 
     def add1 (x y : U32) : Std.Result U32 := do
@@ -1516,8 +1516,8 @@ hf : ∀ (x y : U32), ↑x < 10 → ↑y < 10 → f x y ⦃ x✝ => True ⦄
     example (x y : U32) (h : 2 * x.val + 2 * y.val ≤ U32.max) :
       add1 x y ⦃ _ => True ⦄ := by
       rw [add1]
-      progress? as ⟨ z1, h ⟩ says progress with add_spec' as ⟨ z1, h ⟩
-      progress? as ⟨ z2, h ⟩ says progress with add_spec' as ⟨ z2, h ⟩
+      step? as ⟨ z1, h ⟩ says step with add_spec' as ⟨ z1, h ⟩
+      step? as ⟨ z2, h ⟩ says step with add_spec' as ⟨ z2, h ⟩
 
     /--
     error: unsolved goals
@@ -1534,16 +1534,16 @@ x y : U32
     example (x y : U32) :
       add1 x y ⦃ z => True ⦄ := by
       unfold add1
-      progress
-      swap; progress
+      step
+      swap; step
   end
 
   /- Checking that `add_spec'` went out of scope -/
   example (x y : U32) (h : 2 * x.val + 2 * y.val ≤ U32.max) :
     add1 x y ⦃ _ => True ⦄ := by
     rw [add1]
-    progress? as ⟨ z1, h ⟩ says progress with U32.add_spec as ⟨ z1, h ⟩
-    progress? as ⟨ z2, h ⟩ says progress with U32.add_spec as ⟨ z2, h ⟩
+    step? as ⟨ z1, h ⟩ says step with U32.add_spec as ⟨ z1, h ⟩
+    step? as ⟨ z2, h ⟩ says step with U32.add_spec as ⟨ z2, h ⟩
 end Test
 
 namespace Test
@@ -1555,26 +1555,26 @@ namespace Test
 
   example {i} (l : List α) (h : P i l) :
     f l ⦃ _ => True ⦄ := by
-    progress? as ⟨ b ⟩ says progress with f_spec as ⟨ b ⟩
+    step? as ⟨ b ⟩ says step with f_spec as ⟨ b ⟩
 
-  /- Progress using a term -/
+  /- Step using a term -/
   example {x: U32}
     (f : U32 → Std.Result Unit)
     (h : ∀ x, f x ⦃ _ => True ⦄):
       f x ⦃ () => True ⦄ := by
-      progress? with (show ∀ x, f x ⦃ _ => True ⦄ by exact h) says progress with(show ∀ x, f x ⦃ _ => True ⦄ by exact h)
+      step? with (show ∀ x, f x ⦃ _ => True ⦄ by exact h) says step with(show ∀ x, f x ⦃ _ => True ⦄ by exact h)
 end Test
 
 namespace Test
   open Std Result
 
-  /- Progress using a term -/
+  /- Step using a term -/
   example (x y : U32) (h : 2 * x.val + 2 * y.val ≤ U32.max) :
     add1 x y ⦃ _ => True ⦄ := by
     rw [add1]
     have h1 := add_spec'
-    progress with h1 as ⟨ z1, h ⟩
-    progress with add_spec' z1 as ⟨ z2, h ⟩
+    step with h1 as ⟨ z1, h ⟩
+    step with add_spec' z1 as ⟨ z2, h ⟩
 
   /- Pretty equality when the output type is unit -/
   /--
@@ -1610,7 +1610,7 @@ info: example
           let c1 ← c >>> 16#i32
           ok c1) ⦃ c' => c'.bv = c.bv >>> 16 ⦄
     := by
-    progress as ⟨ c', _, hc' ⟩ -- we have: `hc' : c'.bv = c.bv >>> 16`
+    step as ⟨ c', _, hc' ⟩ -- we have: `hc' : c'.bv = c.bv >>> 16`
     extract_goal1
     fsimp [hc']
 
@@ -1618,7 +1618,7 @@ info: example
     (do
       let z ← x + y
       ok (x, y, z)) ⦃ x y z => z.val = x.val + y.val ⦄ := by
-    progress as ⟨ z ⟩
+    step as ⟨ z ⟩
     scalar_tac
 
   /- Example with an existential -/
@@ -1637,7 +1637,7 @@ _✝ : ↑z = ↑x + y
   #guard_msgs in
   example (x : U32) (f : U32 → Result U32) (h : ∀ x, f x ⦃ y => ∃ z, z > 0 ∧ y.val = x.val + z ⦄) :
     f x ⦃ y => y.val > x.val ⦄ := by
-    progress as ⟨ y, z ⟩
+    step as ⟨ y, z ⟩
 
   /- Inhabited -/
   def get (x : Option α) : Result α :=
@@ -1659,7 +1659,7 @@ z_post : ↑z = ↑x + ↑y
   -/
   #guard_msgs in
   example (x y : U32) : x + y ⦃ z => z.val = x.val + y.val ⦄  := by
-    progress
+    step
 
   /- When using a function call that outputs nothing, we need to ignore the name
      of the let-binding (`massert` is actually bound by a let-binding below). -/
@@ -1668,16 +1668,16 @@ z_post : ↑z = ↑x + ↑y
       massert (x < 32#u32)
       massert (x < 32#u32)
       x + x) ⦃ _ => True ⦄ := by
-      progress
-      progress
-      progress
+      step
+      step
+      step
 
   -- `Inhabited α` is not necessary: we add it for the purpose of testing
   theorem get_spec {α} [Inhabited α] (x : Option α) (h : x.isSome) : get x ⦃ _ => True ⦄ := by
     cases x <;> grind [get]
 
   example {α} [Inhabited α] (x : Option α) (h : x.isSome) : get x ⦃ _ => True ⦄ := by
-    progress with get_spec
+    step with get_spec
 
   namespace Ntt
     def wfArray (_ : Array U16 256#usize) : Prop := True
@@ -1688,7 +1688,7 @@ z_post : ↑z = ↑x + ↑y
 
     def Spec.nttLayer (a : List U16) (_ : Nat) (len : Nat) (_ : Nat) (_ : 0 < len) : List U16 := a
 
-    @[local progress]
+    @[local step]
     theorem nttLayer_spec
       (peSrc : Array U16 256#usize)
       (k : Usize) (len : Usize)
@@ -1722,19 +1722,19 @@ z_post : ↑z = ↑x + ↑y
       ntt peSrc ⦃ peSrc1 => wfArray peSrc1 ⦄
       := by
       unfold ntt
-      progress
-      progress
-      progress
-      progress
-      progress
-      progress
-      progress
-      progress
-      progress
-      progress
-      progress
-      progress
-      progress
+      step
+      step
+      step
+      step
+      step
+      step
+      step
+      step
+      step
+      step
+      step
+      step
+      step
       assumption
 
     theorem ntt_spec' (peSrc : Std.Array U16 256#usize)
@@ -1742,25 +1742,25 @@ z_post : ↑z = ↑x + ↑y
       ntt peSrc ⦃ peSrc1 => wfArray peSrc1 ⦄
       := by
       unfold ntt
-      progress
-      progress;
-      progress
-      progress
-      progress
-      progress
-      progress
-      progress
-      progress
-      progress
-      progress
-      progress
-      progress
+      step
+      step;
+      step
+      step
+      step
+      step
+      step
+      step
+      step
+      step
+      step
+      step
+      step
       assumption
 
   end Ntt
 
 end Test
 
-end Progress
+end Step
 
 end Aeneas
