backends/lean/Aeneas/Step/Trace.lean
@@ -1,10 +1,10 @@
 import Lean
 open Lean Elab Term Meta
 
-namespace Aeneas.Progress
+namespace Aeneas.Step
 
 -- We can't define and use trace classes in the same file
-initialize registerTraceClass `Progress
-initialize registerTraceClass `ProgressElab
+initialize registerTraceClass `Step
+initialize registerTraceClass `StepElab
 
-end Aeneas.Progress
+end Aeneas.Step
